src/Noninterference/LoggedDisk/TS/ATCD_TS_Log.v
@@ -1,1126 +1,1165 @@
-Require Import Eqdep Lia Framework FSParameters CryptoDiskLayer.
-Require Import BatchOperations Log Specs ATCD_TS_BatchOperations.
+Require Import Eqdep Lia Framework FSParameters FileDiskLayer. (* LoggedDiskLayer TransactionCacheLayer TransactionalDiskLayer. *)
+Require Import FileDiskNoninterference FileDiskRefinement.
+Require Import ATCDLayer FileDisk.TransferProofs ATCD_Simulation ATCD_AOE.
+Require Import Not_Init HSS ATCD_ORS.
+Require Import ATCD_TS_Recovery ATCD_TS_Common ATCD_TS_Operations  ATCD_TS_BatchOperations.
 
+Import FileDiskLayer.
 Set Nested Proofs Allowed.
+Opaque File.recover.
 
-Lemma Log_TS_read_header:
-forall u s1 s2 o s1' t,
-exec (CryptoDiskLang) u o s1 
-read_header
-     (Finished s1' t) ->
-exists s2' t,
-exec (CryptoDiskLang) u o s2 
-read_header
-     (Finished s2' t).
+Lemma ATCD_TS_Log_read_header:
+forall n u txns1 txns2 hdr1 hdr2,
+ Termination_Sensitive u
+(@lift_L2 AuthenticationOperation _ TCDLang _
+(@lift_L2 _ _ CachedDiskLang _
+   (|CDDP| Log.read_header)))
+(@lift_L2 AuthenticationOperation _ TCDLang _
+   (@lift_L2 _ _ CachedDiskLang _
+      (|CDDP| Log.read_header)))
+ (Simulation.Definitions.compile
+   ATCD_Refinement
+   (Simulation.Definitions.compile
+ ATC_Refinement
+ (Simulation.Definitions.compile
+    FD.refinement
+    (| Recover |))))
+(refines_valid ATCD_Refinement
+(refines_valid ATC_Refinement AD_valid_state)) 
+(equivalent_for_recovery txns1 txns2 Log.Current_Part hdr1 hdr2)
+(ATCD_reboot_list n).
 Proof.
-unfold read_header in *.
-simpl in *; intros;
-cleanup; repeat invert_exec.
-do 2 eexists; repeat econstructor; eauto.
-Qed.
-
-
-Lemma Log_TS_write_header:
-forall u s1 s2 o s1' t hdr1 hdr2,
-exec (CryptoDiskLang) u o s1 
-(write_header hdr1)
-     (Finished s1' t) ->
-exists s2' t,
-exec (CryptoDiskLang) u o s2 
-(write_header hdr2)
-     (Finished s2' t).
-Proof.
-unfold write_header in *.
-simpl in *; intros;
-cleanup; repeat invert_exec.
-do 2 eexists; repeat econstructor; eauto.
-Qed.
-
-
-
-Lemma Log_TS_check_hash:
-forall u l1 l2 s1 s2 o s1' t h1 h2,
-exec (CryptoDiskLang) u o s1 
-(check_hash l1 h1)
-     (Finished s1' t) ->
-     length l1 = length l2 ->
-consistent_with_upds (snd (fst (fst s2))) (rolling_hash_list hash0 l2)
-(combine (hash0 :: rolling_hash_list hash0 l2) l2) ->
-exists s2' t,
-exec (CryptoDiskLang) u o s2 
-(check_hash l2 h2)
-     (Finished s2' t).
-Proof.
-unfold check_hash in *.
-simpl in *; intros;
-cleanup_no_match; repeat invert_exec_no_match.
-eapply BatchOperations_TS_hash_all with 
-(s2 := s2) (l2:= l2)in H; cleanup_no_match.
-destruct (hash_dec x2 h1);
-repeat invert_exec_no_match;
-destruct (hash_dec x4 h2);
-do 2 eexists; repeat econstructor; eauto;
-destruct (hash_dec x4 h2); try congruence; try econstructor.
-all: eauto.
+ unfold Log.read_header; intros; simpl.
+ eapply ATCD_TS_compositional.
+ intros; apply ATCD_TS_Disk_read; eauto.
+ intuition.
+ intros; apply ATCD_TS_ret.
+ simpl; intros; eauto.
+ repeat invert_exec; eauto.
+ Opaque Log.read_header.
 Qed.
 
 
 
-Lemma Log_read_header_finished:
-forall u s1 o s1' t hdr1 txns1 valid_part1 hdr_blockset1 log_blocksets1,
-
-exec (CryptoDiskLang) u o s1 
-read_header (Finished s1' t) ->
-
-log_rep_explicit Log.Hdr_Synced Log.Synced valid_part1 hdr1 txns1
-hdr_blockset1 log_blocksets1 s1 -> 
-
-s1' = s1 /\ t = hdr1.
+Lemma ATCD_TS_Log_update_header:
+forall n u h1 h2 txns1 txns2 hdr1 hdr2,
+Termination_Sensitive u
+(@lift_L2 AuthenticationOperation _ TCDLang _
+(@lift_L2 _ _ CachedDiskLang _
+   (|CDDP| Log.update_header h1)))
+(@lift_L2 AuthenticationOperation _ TCDLang _
+   (@lift_L2 _ _ CachedDiskLang _
+      (|CDDP| Log.update_header h2)))
+ (Simulation.Definitions.compile
+   ATCD_Refinement
+   (Simulation.Definitions.compile
+ ATC_Refinement
+ (Simulation.Definitions.compile
+    FD.refinement
+    (| Recover |))))
+(refines_valid ATCD_Refinement
+(refines_valid ATC_Refinement AD_valid_state)) 
+(equivalent_for_recovery txns1 txns2
+Log.Current_Part hdr1 hdr2)
+(ATCD_reboot_list n).
 Proof.
-     intros; unfold read_header in *; repeat invert_exec.
-     unfold log_header_rep, log_rep_general, 
-     log_rep_explicit, log_header_block_rep in *; cleanup.
-     repeat cleanup_pairs; eauto.
-Qed.
-
-Lemma Log_read_log: 
-forall u o s s' r hdr txns hdr_blockset log_blocksets valid_part n,
-log_rep_explicit Hdr_Synced Synced valid_part hdr txns hdr_blockset
-        log_blocksets s ->
-exec CryptoDiskLang u o s
-(read_consecutive log_start n) 
-(Finished s' r) ->
-n <= log_length ->
-s' = s /\
-r = firstn n (map fst log_blocksets).
-Proof.
-     intros.
-eapply_fresh read_consecutive_finished in H0; cleanup.
-unfold log_rep_explicit, log_data_blocks_rep in *; cleanup.
-split; eauto.
-eapply Forall2_eq, forall_forall2.
-eapply Forall_forall; intros.
-eapply in_seln_exists in H; cleanup.
-rewrite combine_length_eq in H.
-erewrite seln_combine in H11.
-destruct x; simpl in *; cleanup.
-edestruct H3; eauto; cleanup.
-rewrite seln_firstn in H14.
-erewrite seln_map in H14; eauto. 
-erewrite <- H4 in H14; eauto.
-rewrite H13 in H12; eauto.
-rewrite <- H12, <- H14; eauto.
-all: try lia.
-setoid_rewrite H5; simpl in *; lia.
-all: rewrite firstn_length_l; eauto.
-all: rewrite map_length; setoid_rewrite H5; destruct valid_part; simpl in *; eauto.
-Unshelve.
-exact value0.
-Qed.
-
-Lemma Log_check_hash_finished:
-forall u o s s' r h l,
-exec CryptoDiskLang u o s
-(check_hash l h) 
-(Finished s' r) ->
-(r = true /\ 
-h = rolling_hash hash0 l) \/
-(r = false /\ 
-h <> rolling_hash hash0 l).
-Proof.
-     unfold check_hash; intros; repeat invert_exec; eauto;
-     eapply hash_all_finished in H; cleanup; eauto.
+ intros; simpl.
+ eapply ATCD_TS_compositional.
+ intros; apply ATCD_TS_Log_read_header.
+ 2: shelve.
+ intros.
+ eapply ATCD_TS_Disk_write; intuition.
+ Unshelve.
+ intros.
+ repeat invert_lift2; cleanup.
+ Transparent Log.read_header.
+ unfold Log.read_header in *; repeat invert_exec; eauto.
+ repeat cleanup_pairs; simpl in *; eauto.
+ Opaque Log.read_header Log.update_header.
 Qed.
 
 
-Lemma Log_check_hash_true:
-forall u o s s' r hdr txns hdr_blockset log_blocksets,
-log_rep_explicit Hdr_Synced Synced Current_Part hdr txns hdr_blockset
-        log_blocksets s ->
-exec CryptoDiskLang u o s
-(check_hash (firstn (count (current_part hdr)) (map fst log_blocksets)) (hash (current_part hdr))) 
-(Finished s' r) ->
-r = true.
-Proof.
-     unfold check_hash; intros; repeat invert_exec; eauto.
-     unfold  log_rep_explicit, log_rep_inner, header_part_is_valid in *; cleanup.
-     eapply hash_all_finished in H0; cleanup.
-     clear D. rewrite H6 in n; eauto.
-Qed.
 
-Lemma hashes_in_hashmap_consistent_with_upds:
-forall l m h,
-hashes_in_hashmap m h l ->
-consistent_with_upds m (rolling_hash_list h l)
-  (combine (h :: rolling_hash_list h l) l).
-Proof.
-     induction l; simpl; intros; 
-     cleanup; eauto.
-     unfold consistent; split; eauto.
-     rewrite Mem.upd_nop; eauto; eapply IHl.
-Qed.
+Definition equivalent_for_commit o l_a1 l_v1 l_a2 l_v2 := 
+ fun s1 s2 : state ATCDLang =>
+(forall t : key,
+  In (OpToken ATCDCore (Token2 AuthenticationOperation TCDCore
+     (Token2 (ListOperation (addr * value)) (HorizontalComposition (CacheOperation addr_dec value) CryptoDiskOperation) 
+  (Token2 (CacheOperation addr_dec value) CryptoDiskOperation 
+  (Token1 CryptoOperation 
+  (DiskOperation addr_dec value (fun a => a < disk_size)) (Key t)))))) 
+  o ->
+~ In t (fst (fst (fst (snd (snd (snd s1)))))) ->
+~ In t (fst (fst (fst (snd (snd (snd s2))))))) /\
+(forall r2 : key,
+In (OpToken ATCDCore (Token2 AuthenticationOperation TCDCore
+   (Token2 (ListOperation (addr * value)) (HorizontalComposition (CacheOperation addr_dec value) CryptoDiskOperation) 
+(Token2 (CacheOperation addr_dec value) CryptoDiskOperation 
+(Token1 CryptoOperation 
+(DiskOperation addr_dec value (fun a => a < disk_size)) (Key r2)))))) 
+o -> 
+(forall x,
+consistent_with_upds (snd (fst (fst (snd (snd (snd s1)))))) 
+(firstn x (rolling_hash_list (Log.hash (Log.current_part (Log.decode_header (fst (snd (snd (snd (snd s1))) hdr_block_num))))) 
+(map (encrypt r2) ((addr_list_to_blocks
+(map (Nat.add data_start)
+   l_a1)) ++ l_v1))))
+(firstn x (combine ((Log.hash (Log.current_part (Log.decode_header (fst (snd (snd (snd (snd s1))) hdr_block_num))))) 
+:: rolling_hash_list (Log.hash (Log.current_part (Log.decode_header (fst (snd (snd (snd (snd s1))) hdr_block_num))))) (map (encrypt r2) 
+((addr_list_to_blocks
+(map (Nat.add data_start)
+   l_a1)) ++ l_v1))) 
+   (map (encrypt r2)((addr_list_to_blocks
+   (map (Nat.add data_start)
+      l_a1)) ++ l_v1)))) ->
+consistent_with_upds (snd (fst (fst (snd (snd (snd s2)))))) 
+(firstn x (rolling_hash_list (Log.hash (Log.current_part (Log.decode_header (fst (snd (snd (snd (snd s2))) hdr_block_num))))) 
+(map (encrypt r2) ((addr_list_to_blocks
+(map (Nat.add data_start)
+   l_a2)) ++ l_v2))))
+(firstn x (combine ((Log.hash (Log.current_part (Log.decode_header (fst (snd (snd (snd (snd s2))) hdr_block_num))))) :: 
+rolling_hash_list (Log.hash (Log.current_part (Log.decode_header (fst (snd (snd (snd (snd s2))) hdr_block_num))))) 
+(map (encrypt r2) ((addr_list_to_blocks
+(map (Nat.add data_start)
+   l_a2)) ++ l_v2))) 
+   (map
+   (encrypt r2) ((addr_list_to_blocks
+   (map (Nat.add data_start)
+      l_a2)) ++ l_v2)))))) /\
+      (forall r : key,
+      In (OpToken ATCDCore (Token2 AuthenticationOperation TCDCore
+         (Token2 (ListOperation (addr * value)) (HorizontalComposition (CacheOperation addr_dec value) CryptoDiskOperation) 
+      (Token2 (CacheOperation addr_dec value) CryptoDiskOperation 
+      (Token1 CryptoOperation 
+      (DiskOperation addr_dec value (fun a => a < disk_size)) (Key r)))))) 
+      o ->
+(forall x : nat,
+consistent_with_upds
+ (snd (fst (snd (snd (snd s1)))))
+ (firstn x
+    (map (encrypt r)
+       (addr_list_to_blocks
+          (map (Nat.add data_start)
+             l_a1) ++ l_v1)))
+ (firstn x
+    (map (fun v : value => (r, v))
+       (addr_list_to_blocks
+          (map (Nat.add data_start)
+             l_a1) ++ l_v1))) ->
+consistent_with_upds
+ (snd (fst (snd (snd (snd s2)))))
+ (firstn x
+    (map (encrypt r)
+       (addr_list_to_blocks
+          (map (Nat.add data_start)
+             l_a2) ++ l_v2)))
+ (firstn x
+    (map (fun v : value => (r, v))
+       (addr_list_to_blocks
+          (map (Nat.add data_start)
+             l_a2) ++ l_v2))))).
 
-Lemma in_map_consistent_with_upds:
+
+
+Lemma ATCD_TS_Log_commit_txn:
+forall n u l_a1 l_a2 l_v1 l_v2 txns1 txns2 hdr1 hdr2 lo s1 s2,
+length (addr_list_to_blocks (map (Nat.add data_start) l_a1) ++ l_v1) =
+length (addr_list_to_blocks (map (Nat.add data_start) l_a2) ++ l_v2) ->
+Log.count (Log.current_part hdr2) +(length
+   (addr_list_to_blocks
+      (map (Nat.add data_start) l_a2)) +
+ length l_v2) <= log_length ->
+
+Termination_Sensitive_explicit u lo s1 s2
+(@lift_L2 AuthenticationOperation _ TCDLang _
+(@lift_L2 _ _ CachedDiskLang _
+   (|CDDP| Log.commit_txn
+                (addr_list_to_blocks
+                   (map (Nat.add data_start)
+                      l_a1)) l_v1)))
+(@lift_L2 AuthenticationOperation _ TCDLang _
+   (@lift_L2 _ _ CachedDiskLang _
+      (|CDDP| Log.commit_txn
+                (addr_list_to_blocks
+                   (map (Nat.add data_start)
+                      l_a2)) l_v2)))
+ (Simulation.Definitions.compile
+   ATCD_Refinement
+   (Simulation.Definitions.compile
+ ATC_Refinement
+ (Simulation.Definitions.compile
+    FD.refinement
+    (| Recover |))))
+(refines_valid ATCD_Refinement
+(refines_valid ATC_Refinement AD_valid_state)) 
+(fun s1 s2 => 
+equivalent_for_recovery txns1 txns2 Log.Current_Part hdr1 hdr2 s1 s2 /\
+equivalent_for_commit (seln lo 0 []) l_a1 l_v1 l_a2 l_v2 s1 s2)
+(ATCD_reboot_list n).
+Proof.
+ Transparent Log.commit_txn.
+ Opaque Log.update_header.
+ unfold Log.commit_txn; intros; simpl.
+ eapply ATCD_TS_explicit_compositional.
+ intros; eapply TS_explicit_eqv_impl.
+ intros; eapply TS_explicit_to_TS.
+ intros; apply ATCD_TS_Log_read_header.
+ intros; cleanup; eauto.
+ 2: shelve.
+
+ intros. 
+ repeat invert_lift2; cleanup_no_match.
+ unfold equivalent_for_recovery in *; cleanup_no_match.
+ eapply Log_read_header_finished in H17; eauto.
+ eapply Log_read_header_finished in H11; eauto.
+ cleanup_no_match.
+ repeat cleanup_pairs; simpl in *.
+ eapply ATCD_TS_explicit_compositional.
+ intros. eapply TS_explicit_eqv_impl.
+ intros; apply ATCD_TS_Crypto_getkey.
+ shelve.
+ 2: shelve.
+
+ simpl; intros.
+ repeat invert_exec; cleanup_no_match.
+ intros; eapply TS_explicit_to_TS.
+ eapply ATCD_TS_compositional.
+ intros; eapply TS_eqv_impl.
+ apply ATCD_TS_BatchOperations_encrypt_all; eauto.
+ simpl; shelve.
+ 2: shelve.
+
+ intros.
+ repeat invert_lift2; cleanup_no_match.
+ eapply BatchOperations.encrypt_all_finished in H32; eauto.
+ eapply BatchOperations.encrypt_all_finished in H20; eauto.
+ cleanup_no_match.
+ repeat cleanup_pairs; simpl in *.
+ eapply ATCD_TS_compositional.
+ intros; eapply TS_eqv_impl.
+ intros; apply ATCD_TS_BatchOperations_hash_all; eauto.
+ repeat rewrite map_length; eauto.
+ shelve.
+ 2: shelve.
+
+ simpl; intros.
+ repeat invert_lift2; cleanup_no_match.
+ eapply BatchOperations.hash_all_finished in H36; eauto.
+ eapply BatchOperations.hash_all_finished in H29; eauto.
+ repeat cleanup_pairs; simpl in *.
+ eapply ATCD_TS_compositional.
+ intros; eapply TS_eqv_impl.
+ intros; apply ATCD_TS_BatchOperations_write_batch; eauto.
+ all: repeat rewrite seq_length; repeat rewrite map_length; eauto.
+ {
+    eapply Forall_forall; intros.
+    apply in_seq in H2.
+    rewrite app_length in H2.
+    rewrite data_fits_in_disk.
+    rewrite data_start_where_log_ends.
+    lia.
+ }
+ shelve.
+ 2: shelve.
+
+ simpl; intros.
+ repeat invert_lift2; cleanup_no_match.
+ eapply BatchOperations.write_consecutive_finished in H40; eauto.
+ eapply BatchOperations.write_consecutive_finished in H33; eauto.
+ all: repeat rewrite seq_length; repeat rewrite  map_length; eauto.
+ repeat cleanup_pairs; simpl in *.
+ cleanup_no_match.
+ eapply ATCD_TS_compositional.
+ intros; apply ATCD_TS_Log_update_header; eauto.
+ intros; apply ATCD_TS_Disk_sync; eauto.
+ simpl; shelve.
+
+ Unshelve.
+ {
+    instantiate (1:= fun r1 r2 s1 s2 =>
+    equivalent_for_recovery txns1 txns2 Log.Current_Part hdr1 hdr2 s1 s2 /\
+    equivalent_for_commit (seln lo 0 []) l_a1 l_v1 l_a2 l_v2 s1 s2).
+    simpl; intros.
+    repeat invert_lift2; cleanup_no_match.
+    unfold equivalent_for_recovery in *; cleanup_no_match.
+    eapply Log_read_header_finished in H17; eauto.
+    eapply Log_read_header_finished in H11; eauto.
+    cleanup_no_match; intuition eauto.
+    do 2 eexists; intuition eauto.
+    repeat cleanup_pairs; eauto.
+ }
+ 5:{
+    simpl; intuition eauto.
+    unfold equivalent_for_commit in *; cleanup_no_match.
+    repeat cleanup_pairs; eauto.
+    simpl in *.
+    setoid_rewrite H1 in H8.
+    eapply H8; eauto.
+ }
+ {
+    instantiate (1:= fun r1 r2 s6 s7 =>
+    equivalent_for_recovery txns1 
+txns2 Log.Current_Part hdr1 
+hdr2 s6 s7 /\
+(forall r5 : key,
+In
+  (OpToken ATCDCore
+     (Token2 AuthenticationOperation TCDCore
+        (Token2 (ListOperation (addr * value))
+           (HorizontalComposition (CacheOperation addr_dec value)
+              CryptoDiskOperation)
+           (Token2 (CacheOperation addr_dec value) CryptoDiskOperation
+              (Token1 CryptoOperation
+                 (DiskOperation addr_dec value (fun a : addr => a < disk_size))
+                 (Key r5)))))) (seln lo 0 []) ->
+forall x : nat,
+consistent_with_upds (snd (fst (fst (snd (snd (snd s6))))))
+  (firstn x
+     (rolling_hash_list (Log.hash (Log.current_part (Log.decode_header (fst (snd (snd (snd (snd s6))) hdr_block_num)))))
+        (map (encrypt r5)
+           (addr_list_to_blocks (map (Nat.add data_start) l_a1) ++ l_v1))))
+  (firstn x
+     match
+       map (encrypt r5)
+         (addr_list_to_blocks (map (Nat.add data_start) l_a1) ++ l_v1)
+     with
+     | [] => []
+     | y :: tl' =>
+         (Log.hash (Log.current_part (Log.decode_header (fst (snd (snd (snd (snd s6))) hdr_block_num)))), y)
+         :: combine
+              (rolling_hash_list (Log.hash (Log.current_part (Log.decode_header (fst (snd (snd (snd (snd s6))) hdr_block_num)))))
+                 (map (encrypt r5)
+                    (addr_list_to_blocks (map (Nat.add data_start) l_a1) ++ l_v1)))
+              tl'
+     end) ->
+consistent_with_upds (snd (fst (fst (snd (snd (snd s7))))))
+  (firstn x
+     (rolling_hash_list (Log.hash (Log.current_part (Log.decode_header (fst (snd (snd (snd (snd s7))) hdr_block_num)))))
+        (map (encrypt r5)
+           (addr_list_to_blocks (map (Nat.add data_start) l_a2) ++ l_v2))))
+  (firstn x
+     match
+       map (encrypt r5)
+         (addr_list_to_blocks (map (Nat.add data_start) l_a2) ++ l_v2)
+     with
+     | [] => []
+     | y :: tl' =>
+         (Log.hash (Log.current_part (Log.decode_header (fst (snd (snd (snd (snd s7))) hdr_block_num)))), y)
+         :: combine
+              (rolling_hash_list (Log.hash (Log.current_part (Log.decode_header (fst (snd (snd (snd (snd s7))) hdr_block_num)))))
+                 (map (encrypt r5)
+                    (addr_list_to_blocks (map (Nat.add data_start) l_a2) ++ l_v2)))
+              tl'
+     end)) /\
+(forall r : key,
+        In
+          (OpToken ATCDCore
+             (Token2 AuthenticationOperation TCDCore
+                (Token2 (ListOperation (addr * value))
+                   (HorizontalComposition (CacheOperation addr_dec value)
+                      CryptoDiskOperation)
+                   (Token2 (CacheOperation addr_dec value) CryptoDiskOperation
+                      (Token1 CryptoOperation
+                         (DiskOperation addr_dec value
+                            (fun a : addr => a < disk_size)) 
+                         (Key r)))))) (seln lo 0 []) ->
+        forall x : nat,
+        consistent_with_upds (snd (fst (snd (snd (snd s6)))))
+          (firstn x
+             (map (encrypt r)
+                (addr_list_to_blocks (map (Nat.add data_start) l_a1) ++ l_v1)))
+          (firstn x
+             (map (fun v : value => (r, v))
+                (addr_list_to_blocks (map (Nat.add data_start) l_a1) ++ l_v1))) ->
+        consistent_with_upds (snd (fst (snd (snd (snd s7)))))
+          (firstn x
+             (map (encrypt r)
+                (addr_list_to_blocks (map (Nat.add data_start) l_a2) ++ l_v2)))
+          (firstn x
+             (map (fun v : value => (r, v))
+                (addr_list_to_blocks (map (Nat.add data_start) l_a2) ++ l_v2))))).
+
+    simpl; eauto.
+    intros; repeat invert_exec.
+    cleanup_no_match; simpl in *.
+    intuition eauto.
+
+    repeat cleanup_pairs; simpl in *.
+    unfold equivalent_for_recovery in *; cleanup_no_match.
+    simpl in *; do 2 eexists; intuition eauto.
+    do 2 eexists; split.
+    eapply RepImplications.log_rep_explicit_new_key; eauto.
+    eauto.
+    do 2 eexists; split.
+    eapply RepImplications.log_rep_explicit_new_key; eauto.
+    eauto.
+
+    all: unfold equivalent_for_commit in *; 
+    cleanup_no_match; simpl in *;
+    intuition.
+ }
+ 5: {
+    simpl; intros; eauto.
+    cleanup_no_match; intuition eauto.
+    setoid_rewrite H1 in H6; simpl in *;
+    eapply H6; intuition eauto.
+    simpl; intuition.
+ }
+ 7: {
+    instantiate (5:= fun _ _ s19 s20 =>
+    equivalent_for_recovery txns1 
+      txns2 Log.Current_Part 
+      hdr1 hdr2 s19 s20 /\
+      (forall x : nat,
+      consistent_with_upds (snd (fst (fst (snd (snd (snd s19))))))
+        (firstn x
+           (rolling_hash_list (Log.hash (Log.current_part (Log.decode_header (fst (snd (snd (snd (snd s19))) hdr_block_num)))))
+              (map (encrypt r2) (addr_list_to_blocks (map (Nat.add data_start) l_a1) ++ l_v1))))
+        (firstn x
+           match
+             map (encrypt r2) (addr_list_to_blocks (map (Nat.add data_start) l_a1) ++ l_v1)
+           with
+           | [] => []
+           | y :: tl' =>
+               (Log.hash (Log.current_part (Log.decode_header (fst (snd (snd (snd (snd s19))) hdr_block_num)))), y)
+               :: combine
+                    (rolling_hash_list (Log.hash (Log.current_part (Log.decode_header (fst (snd (snd (snd (snd s19))) hdr_block_num)))))
+                       (map (encrypt r2)
+                          (addr_list_to_blocks (map (Nat.add data_start) l_a1) ++ l_v1))) tl'
+           end) ->
+      consistent_with_upds (snd (fst (fst (snd (snd (snd s20))))))
+        (firstn x
+           (rolling_hash_list (Log.hash (Log.current_part (Log.decode_header (fst (snd (snd (snd (snd s20))) hdr_block_num)))))
+              (map (encrypt r2) (addr_list_to_blocks (map (Nat.add data_start) l_a2) ++ l_v2))))
+        (firstn x
+           match
+             map (encrypt r2) (addr_list_to_blocks (map (Nat.add data_start) l_a2) ++ l_v2)
+           with
+           | [] => []
+           | y :: tl' =>
+               (Log.hash (Log.current_part (Log.decode_header (fst (snd (snd (snd (snd s20))) hdr_block_num)))), y)
+               :: combine
+                    (rolling_hash_list (Log.hash (Log.current_part (Log.decode_header (fst (snd (snd (snd (snd s20))) hdr_block_num)))))
+                       (map (encrypt r2)
+                          (addr_list_to_blocks (map (Nat.add data_start) l_a2) ++ l_v2))) tl'
+           end))).
+    simpl; eauto.
+    intros; intuition eauto.
+    unfold equivalent_for_recovery, Log.log_rep_explicit,
+    Log.log_header_block_rep in H10; cleanup_no_match; intuition.
+ }
+ {
+    simpl; eauto.
+    intros;
+    repeat invert_lift2; cleanup_no_match.
+    eapply BatchOperations.encrypt_all_finished in H26.
+    eapply BatchOperations.encrypt_all_finished in H34.
+    cleanup_no_match.
+    repeat cleanup_pairs; simpl in *.
+    intuition eauto.
+
+    repeat cleanup_pairs; simpl in *.
+    unfold equivalent_for_recovery in *; cleanup_no_match.
+    simpl in *; do 2 eexists; intuition eauto.
+    do 2 eexists; split.
+    eapply RepImplications.log_rep_explicit_consistent_with_upds; eauto.
+    eauto.
+    do 2 eexists; split.
+    eapply RepImplications.log_rep_explicit_consistent_with_upds; eauto.
+    eauto.
+
+    setoid_rewrite H1 in H10; 
+    simpl in *. 
+    eapply H10; eauto.
+    simpl; intuition.
+ }
+ 7: {
+    simpl; eauto.
+    instantiate (5:= fun _ _ s19 s20 =>
+    equivalent_for_recovery txns1 
+      txns2 Log.Current_Part 
+      hdr1 hdr2 s19 s20).
+    simpl; eauto.
+ }
+ {
+    simpl; intros;
+    repeat invert_lift2; cleanup_no_match.
+    eapply BatchOperations.hash_all_finished in H30.
+    eapply BatchOperations.hash_all_finished in H37.
+    cleanup_no_match.
+    repeat cleanup_pairs; simpl in *.
+    unfold equivalent_for_recovery in *; cleanup_no_match.
+    simpl in *; do 2 eexists; intuition eauto.
+    do 2 eexists; split.
+    eapply RepImplications.log_rep_explicit_consistent_with_upds_hashmap; eauto.
+    eauto.
+    do 2 eexists; split.
+    eapply RepImplications.log_rep_explicit_consistent_with_upds_hashmap; eauto.
+    eauto.
+ }
+ {
+    simpl; intros;
+    repeat invert_lift2; cleanup_no_match.
+    eapply BatchOperations.write_consecutive_finished in H33.
+    eapply BatchOperations.write_consecutive_finished in H40.
+    all: try solve [rewrite seq_length; eauto].
+    cleanup_no_match.
+    repeat cleanup_pairs; simpl in *.
+    admit.
+ }
+ 9: {
+    simpl; intros;
+    repeat invert_lift2; cleanup_no_match.
+    eapply Specs.update_header_finished in H38; eauto.
+    eapply Specs.update_header_finished in H44; eauto.
+    cleanup_no_match.
+    repeat cleanup_pairs; simpl in *.
+    admit.
+ }
+ Opaque Log.commit_txn.
+Admitted.
+
+Lemma consistent_with_upds_firstn:
 forall A AEQ V l1 l2 (m: @mem A AEQ V),
-Forall2 (fun a v => m a = Some v) l1 l2 ->
-consistent_with_upds m l1 l2.
+consistent_with_upds m l1 l2 ->
+forall n, consistent_with_upds m (firstn n l1) (firstn n l2).
 Proof.
-     induction l1; destruct l2; simpl; intros; 
-     cleanup; eauto; inversion H; cleanup.
-     unfold consistent; split; eauto.
-     rewrite Mem.upd_nop; eauto; eapply IHl.
+ induction l1; destruct n;
+ simpl; intros; 
+ destruct l2; eauto.
+ simpl in *; cleanup; intuition eauto.
 Qed.
 
-Lemma Log_TS_read_encrypted_log:
-forall u s1 s2 o s1' t hdr1 hdr2 txns1 txns2
-valid_part hdr_blockset1 hdr_blockset2 
-log_blocksets1 log_blocksets2,
-
-exec (CryptoDiskLang) u o s1 
-read_encrypted_log
-     (Finished s1' t) ->
-
-log_rep_explicit Log.Hdr_Synced Log.Synced valid_part hdr1 txns1
-hdr_blockset1 log_blocksets1 s1 -> 
-log_rep_explicit Log.Hdr_Synced Log.Synced valid_part hdr2 txns2
-hdr_blockset2 log_blocksets2 s2 -> 
-
-(Log.hash (Log.current_part hdr1) <>
-rolling_hash hash0
-     (firstn (Log.count (Log.current_part hdr1)) (map fst log_blocksets1)) <->
-Log.hash (Log.current_part hdr2) <>
-     rolling_hash hash0
-          (firstn (Log.count (Log.current_part hdr2)) (map fst log_blocksets2))) ->
-
-Forall2
-(fun rec1 rec2 : Log.txn_record =>
-     Log.start rec1 = Log.start rec2 /\
-     Log.addr_count rec1 = Log.addr_count rec2 /\
-     Log.data_count rec1 = Log.data_count rec2)
-(map Log.record txns1)
-(map Log.record txns2) ->
-
-consistent_with_upds (snd (fst (fst s2)))
-  (rolling_hash_list hash0
-     (firstn (count (current_part hdr2)) (map fst log_blocksets2)))
-  (combine
-     (hash0
-      :: rolling_hash_list hash0
-           (firstn (count (current_part hdr2)) (map fst log_blocksets2)))
-     (firstn (count (current_part hdr2)) (map fst log_blocksets2))) ->
-
-consistent_with_upds (snd (fst (fst s2)))
-  (rolling_hash_list hash0
-     (firstn (count (old_part hdr2)) (map fst log_blocksets2)))
-  (combine
-     (hash0
-      :: rolling_hash_list hash0
-           (firstn (count (old_part hdr2)) (map fst log_blocksets2)))
-     (firstn (count (old_part hdr2)) (map fst log_blocksets2))) ->
-
-(valid_part = Old_Part -> count (current_part hdr1) = count (current_part hdr2)) ->
-
-exists s2' t,
-exec (CryptoDiskLang) u o s2 
-read_encrypted_log
-     (Finished s2' t).
+Lemma ATCD_TS_Log_read_encrypted_log:
+forall n u txns1 txns2 hdr1 hdr2,
+Termination_Sensitive u 
+(@lift_L2 AuthenticationOperation _ TCDLang _
+(@lift_L2 _ _ CachedDiskLang _
+   (|CDDP| Log.read_encrypted_log)))
+(@lift_L2 AuthenticationOperation _ TCDLang _
+   (@lift_L2 _ _ CachedDiskLang _
+      (|CDDP| Log.read_encrypted_log)))
+ (Simulation.Definitions.compile
+   ATCD_Refinement
+   (Simulation.Definitions.compile
+ ATC_Refinement
+ (Simulation.Definitions.compile
+    FD.refinement
+    (| Recover |))))
+(refines_valid ATCD_Refinement
+(refines_valid ATC_Refinement AD_valid_state)) 
+(equivalent_for_recovery txns1 txns2 Log.Current_Part hdr1 hdr2)
+(ATCD_reboot_list n).
 Proof.
-unfold read_encrypted_log in *.
-simpl in *; intros;
-cleanup_no_match; repeat invert_exec_no_match.
-{
-     eapply_fresh Log_TS_read_header with (s2:= s2) in H; cleanup_no_match.
-eapply_fresh Log_read_header_finished in H; eauto.
-eapply_fresh Log_read_header_finished in H10; eauto.
-cleanup_no_match.
+ Opaque Log.read_encrypted_log.
+ unfold Termination_Sensitive, ATCD_reboot_list; destruct n; intros; repeat invert_exec.
+ {
+    repeat invert_lift2; cleanup.
+    unfold equivalent_for_recovery in *; cleanup.
+    eapply Log_TS_read_encrypted_log in H8; eauto; cleanup.
 
-assume (A: (count (current_part hdr1) = count (current_part hdr2))).
+    destruct s2, s0, s2.
+    eexists (RFinished _ _); repeat econstructor; eauto.
+    repeat apply lift2_exec_step; eauto.
 
-eapply_fresh BatchOperations_TS_read_consecutive with (s2:= s2) in H7; cleanup_no_match.
-unfold log_header_rep, log_rep_general in *; cleanup_no_match.
-eapply_fresh Log_read_log in H7; eauto.
-eapply_fresh Log_read_log in H11; eauto.
-2: eauto.
-cleanup_no_match.
+    exact ATCDLang.
+    unfold Log.log_rep_explicit,
+    Log.log_rep_inner,
+    Log.header_part_is_valid  in *; logic_clean.
+    rewrite <- H6 at 1; clear H6.
+    rewrite H27, H38.
+    intuition.
 
-eapply_fresh Log_TS_check_hash with (s2 := s2) in H8; cleanup_no_match.
+    unfold Log.log_rep_explicit,
+    Log.log_rep_inner,
+    Log.header_part_is_valid  in *; logic_clean.
+    eapply hashes_in_hashmap_consistent_with_upds; eauto.
 
-eapply_fresh Log_check_hash_finished in H8; eauto; cleanup_no_match.
-eapply_fresh Log_check_hash_finished in H12; eauto; cleanup_no_match.
+    unfold Log.log_rep_explicit,
+    Log.log_rep_inner,
+    Log.header_part_is_valid  in *; logic_clean.
+    eapply hashes_in_hashmap_consistent_with_upds; eauto.
 
-repeat split_ors; logic_clean; subst; try congruence.
+    (** Check this. Does alld count hashes are always in hashmap? Does it have to be? **)
+    admit.
+ }
+ {
+    repeat invert_lift2; cleanup.
+    unfold equivalent_for_recovery in *; cleanup.
+    eapply_fresh Specs.read_encrypted_log_crashed in H8; eauto.
+    cleanup.
+    eapply Log_TS_read_encrypted_log_crashed in H8; eauto; cleanup.
+    eapply_fresh Specs.read_encrypted_log_crashed in H8; eauto.
+    cleanup.
 
-do 2 eexists; repeat econstructor; eauto.
-simpl; repeat invert_exec_no_match; repeat econstructor.
+    destruct s2, s0, s2.
+    edestruct ATCD_TS_recovery.
+    3: eauto.
+    3: eapply equivalent_for_recovery_after_reboot.
+    all: try solve [unfold AD_valid_state, 
+    refines_valid, FD_valid_state; 
+    intros; simpl; eauto].
+    shelve.
 
-exfalso; destruct H2; apply H2; eauto.
-exfalso; apply H2; eauto.
+    eexists (Recovered _); econstructor; eauto.
+    repeat eapply lift2_exec_step_crashed; eauto.
 
-repeat invert_exec_no_match.
-assume (A0: (count (old_part hdr1) = count (old_part hdr2))).
-eapply_fresh BatchOperations_TS_read_consecutive with (s2:= x1) in H9; cleanup_no_match.
+    unfold Log.log_rep_explicit,
+    Log.log_rep_inner,
+    Log.header_part_is_valid  in *; logic_clean.
+    rewrite <- H6 at 1; clear H6.
+    rewrite H32, H43.
+    intuition.
 
-do 2 eexists; repeat econstructor; eauto.
-simpl.
-repeat econstructor; eauto.
+    unfold Log.log_rep_explicit,
+    Log.log_rep_inner,
+    Log.header_part_is_valid  in *; logic_clean.
+    intros.
+    eapply consistent_with_upds_firstn; eapply hashes_in_hashmap_consistent_with_upds; eauto.
 
-pose proof data_fits_in_disk.
-pose proof data_start_where_log_ends.
-pose proof all_fits_to_data_region.
-unfold log_header_rep, log_rep_general,  log_rep_explicit in *; logic_clean.
-lia.
+    unfold Log.log_rep_explicit,
+    Log.log_rep_inner,
+    Log.header_part_is_valid  in *; logic_clean.
+    intros.
+    eapply consistent_with_upds_firstn; eapply hashes_in_hashmap_consistent_with_upds; eauto.
 
-repeat rewrite firstn_length_l; eauto.
-rewrite map_length.
-unfold  log_rep_explicit in *; logic_clean.
-setoid_rewrite H14; eauto.
+    (** Check this. Does alld count hashes are always in hashmap? Does it have to be? **)
+    admit.
 
-rewrite map_length.
-unfold  log_rep_explicit in *; logic_clean.
-setoid_rewrite H20; eauto.
-
-eauto.
-
-pose proof data_fits_in_disk.
-pose proof data_start_where_log_ends.
-pose proof all_fits_to_data_region.
-unfold log_header_rep, log_rep_general,  log_rep_explicit in *; logic_clean.
-lia.
-
-pose proof data_fits_in_disk.
-pose proof data_start_where_log_ends.
-pose proof all_fits_to_data_region.
-unfold log_header_rep, log_rep_general,  log_rep_explicit in *; logic_clean.
-lia.
-
-pose proof data_fits_in_disk.
-pose proof data_start_where_log_ends.
-pose proof all_fits_to_data_region.
-unfold log_header_rep, log_rep_general,  log_rep_explicit in *; logic_clean.
-lia.
-}
-Unshelve.
-{
-     unfold log_rep_explicit, log_rep_inner, header_part_is_valid, txns_valid in *; logic_clean.
-     rewrite <- H17, <- H29 in *; clear H17 H29.
-     rewrite map_map in *.
-     destruct valid_part; eauto.
-     admit. (* Needs lemma *)
-}
-{
-     unfold log_rep_explicit, log_rep_inner, header_part_is_valid, txns_valid in *; logic_clean.
-     rewrite <- H21, <- H33 in *; clear H21 H33.
-     rewrite map_map in *.
-     destruct valid_part; eauto.
-     rewrite <- A in *; clear A.
-     eapply Log_check_hash_true in H8; try congruence.
-     admit. (* Needs lemma *)
-}
+    intuition congruence.
+ }
+ Unshelve.
+ all: try solve [exact ATCDLang].
+ 5:{
+    repeat cleanup_pairs.
+    instantiate (1:= hdr2).
+    instantiate (1:= hdr1).
+    instantiate (1:= txns2).
+    instantiate (1:= txns1).
+    unfold equivalent_for_recovery; simpl; eexists (_, (_, _)), (_, (_, _));
+    simpl; intuition eauto.
+    do 2 eexists; intuition eauto; try congruence.
+    eapply RepImplications.log_rep_explicit_subset_hashmap; eauto.
+    do 2 eexists; intuition eauto; try congruence.
+    eapply RepImplications.log_rep_explicit_subset_hashmap; eauto.
+ }
 Admitted.
 
 
 
-
-Lemma Log_TS_decrypt_txn:
-forall u record1 record2 s1 s2 o s1' t log1 log2,
-
-exec (CryptoDiskLang) u o s1 
-(decrypt_txn record1 log1)
-     (Finished s1' t) ->
-
+Lemma ATCD_TS_Log_decrypt_txn:
+forall rec1 log1 rec2 log2 n u txns1 txns2 hdr1 hdr2,
 length
-     (firstn (addr_count record1 + data_count record1)
-        (skipn (start record1) log1)) =
+(firstn (Log.addr_count rec1 + Log.data_count rec1)
+   (skipn (Log.start rec1) log1)) =
 length
-     (firstn (addr_count record2 + data_count record2)
-        (skipn (start record2) log2)) ->
-   
-consistent_with_upds (snd (fst s2))
-     (firstn (addr_count record2 + data_count record2)
-        (skipn (start record2) log2))
-     (map (fun ev : value => (key record2, decrypt (key record2) ev))
-        (firstn (addr_count record2 + data_count record2)
-           (skipn (start record2) log2))) ->
-
-exists s2' t,
-exec (CryptoDiskLang) u o s2 (decrypt_txn record2 log2) (Finished s2' t).
+(firstn (Log.addr_count rec2 + Log.data_count rec2)
+   (skipn (Log.start rec2) log2))  -> 
+Termination_Sensitive u 
+(@lift_L2 AuthenticationOperation _ TCDLang _
+(@lift_L2 _ _ CachedDiskLang _
+   (|CDDP| Log.decrypt_txn rec1 log1)))
+(@lift_L2 AuthenticationOperation _ TCDLang _
+   (@lift_L2 _ _ CachedDiskLang _
+      (|CDDP| Log.decrypt_txn rec2 log2)))
+ (Simulation.Definitions.compile
+   ATCD_Refinement
+   (Simulation.Definitions.compile
+ ATC_Refinement
+ (Simulation.Definitions.compile
+    FD.refinement
+    (| Recover |))))
+(refines_valid ATCD_Refinement
+(refines_valid ATC_Refinement AD_valid_state)) 
+(fun s1 s2 => equivalent_for_recovery txns1 txns2 Log.Current_Part hdr1 hdr2 s1 s2 /\
+consistent_with_upds (snd (fst (snd (snd (snd s2)))))
+(firstn (Log.addr_count rec2 + Log.data_count rec2)
+ (skipn (Log.start rec2) log2))
+(map (fun ev : value => (Log.key rec2, decrypt (Log.key rec2) ev))
+ (firstn (Log.addr_count rec2 + Log.data_count rec2)
+    (skipn (Log.start rec2) log2))))
+(ATCD_reboot_list n).
 Proof.
-     unfold decrypt_txn; intros; repeat invert_exec.
-     eapply BatchOperations_TS_decrypt_all with (s2:= s2) (k2:= (key record2)) 
-     (l2 := firstn (addr_count record2 + data_count record2)
-     (skipn (start record2) log2)) in H; cleanup.
-     do 2 eexists; repeat econstructor; eauto.
-     all: eauto.
+ Opaque Log.decrypt_txn.
+ unfold Termination_Sensitive, ATCD_reboot_list; destruct n; intros; repeat invert_exec.
+ {
+    repeat invert_lift2; cleanup.
+    unfold equivalent_for_recovery in *; cleanup.
+    destruct s2, s0, s2.
+    eapply Log_TS_decrypt_txn with (record2:= rec2) (log2:= log2) in H8; eauto; cleanup.
+
+    eexists (RFinished _ _); repeat econstructor; eauto.
+    repeat apply lift2_exec_step; eauto.
+    exact ATCDLang.
+ }
+ {
+    repeat invert_lift2; cleanup.
+    unfold equivalent_for_recovery in *; cleanup.
+    eapply_fresh Specs.decrypt_txn_crashed in H8; eauto.
+    cleanup.
+    eapply Log_TS_decrypt_txn_crashed in H8; eauto; cleanup.
+    eapply_fresh Specs.decrypt_txn_crashed in H8; eauto.
+    cleanup.
+
+    destruct s2, s0, s2.
+    edestruct ATCD_TS_recovery.
+    3: eauto.
+    3: eapply equivalent_for_recovery_after_reboot.
+    all: try solve [unfold AD_valid_state, 
+    refines_valid, FD_valid_state; 
+    intros; simpl; eauto].
+    shelve.
+
+    eexists (Recovered _); econstructor; eauto.
+    repeat eapply lift2_exec_step_crashed; eauto.
+ }
+ Unshelve.
+ all: try solve [exact ATCDLang].
+ 5:{
+    repeat cleanup_pairs.
+    instantiate (1:= hdr2).
+    instantiate (1:= hdr1).
+    instantiate (1:= txns2).
+    instantiate (1:= txns1).
+    unfold equivalent_for_recovery; simpl; eexists (_, (_, _)), (_, (_, _));
+    simpl; intuition eauto.
+    do 2 eexists; intuition eauto; try congruence.
+    eapply RepImplications.log_rep_explicit_consistent_with_upds; eauto.
+    do 2 eexists; intuition eauto; try congruence.
+    eapply RepImplications.log_rep_explicit_consistent_with_upds; eauto.
+ }
+Qed.
+
+Definition apply_txn_precondition log1 log2 rec1 rec2 :=
+ length
+ (firstn (Log.addr_count rec1 + Log.data_count rec1)
+    (skipn (Log.start rec1) log1)) =
+length
+ (firstn (Log.addr_count rec2 + Log.data_count rec2)
+    (skipn (Log.start rec2) log2))  /\
+
+length
+ (firstn (Log.data_count rec1)
+    (blocks_to_addr_list
+       (firstn (Log.addr_count rec1)
+          (map (decrypt (Log.key rec1))
+             (firstn (Log.addr_count rec1 + Log.data_count rec1)
+                (skipn (Log.start rec1) log1)))))) =
+length
+ (firstn (Log.data_count rec2)
+    (blocks_to_addr_list
+       (firstn (Log.addr_count rec2)
+          (map (decrypt (Log.key rec2))
+             (firstn (Log.addr_count rec2 + Log.data_count rec2)
+                (skipn (Log.start rec2) log2)))))) /\
+length
+ (skipn (Log.addr_count rec1)
+    (map (decrypt (Log.key rec1))
+       (firstn (Log.addr_count rec1 + Log.data_count rec1)
+          (skipn (Log.start rec1) log1)))) =
+length
+ (skipn (Log.addr_count rec2)
+    (map (decrypt (Log.key rec2))
+       (firstn (Log.addr_count rec2 + Log.data_count rec2)
+          (skipn (Log.start rec2) log2)))) /\
+
+length
+  (firstn (Log.data_count rec1)
+     (blocks_to_addr_list
+        (firstn (Log.addr_count rec1)
+           (map (decrypt (Log.key rec1))
+              (firstn (Log.addr_count rec1 + Log.data_count rec1)
+                 (skipn (Log.start rec1) log1)))))) =
+length
+  (skipn (Log.addr_count rec1)
+     (map (decrypt (Log.key rec1))
+        (firstn (Log.addr_count rec1 + Log.data_count rec1)
+           (skipn (Log.start rec1) log1)))) /\
+
+length
+ (firstn (Log.data_count rec2)
+    (blocks_to_addr_list
+       (firstn (Log.addr_count rec2)
+          (map (decrypt (Log.key rec2))
+             (firstn (Log.addr_count rec2 + Log.data_count rec2)
+                (skipn (Log.start rec2) log2)))))) =
+length
+ (skipn (Log.addr_count rec2)
+    (map (decrypt (Log.key rec2))
+       (firstn (Log.addr_count rec2 + Log.data_count rec2)
+          (skipn (Log.start rec2) log2)))) /\
+
+Forall (fun a : nat => a < disk_size)
+ (firstn (Log.data_count rec2)
+    (blocks_to_addr_list
+       (firstn (Log.addr_count rec2)
+          (map (decrypt (Log.key rec2))
+             (firstn (Log.addr_count rec2 + Log.data_count rec2)
+                (skipn (Log.start rec2) log2)))))).
+
+Lemma ATCD_TS_Log_apply_txn:
+forall rec1 log1 rec2 log2 n u txns1 txns2 hdr1 hdr2,
+apply_txn_precondition log1 log2 rec1 rec2 ->
+
+Termination_Sensitive u 
+(@lift_L2 AuthenticationOperation _ TCDLang _
+(@lift_L2 _ _ CachedDiskLang _
+   (|CDDP| Log.apply_txn rec1 log1)))
+(@lift_L2 AuthenticationOperation _ TCDLang _
+   (@lift_L2 _ _ CachedDiskLang _
+      (|CDDP| Log.apply_txn rec2 log2)))
+ (Simulation.Definitions.compile
+   ATCD_Refinement
+   (Simulation.Definitions.compile
+ ATC_Refinement
+ (Simulation.Definitions.compile
+    FD.refinement
+    (| Recover |))))
+(refines_valid ATCD_Refinement
+(refines_valid ATC_Refinement AD_valid_state)) 
+(fun s1 s2 => equivalent_for_recovery txns1 txns2 Log.Current_Part hdr1 hdr2 s1 s2 /\
+consistent_with_upds (snd (fst (snd (snd (snd s2)))))
+(firstn (Log.addr_count rec2 + Log.data_count rec2)
+ (skipn (Log.start rec2) log2))
+(map (fun ev : value => (Log.key rec2, decrypt (Log.key rec2) ev))
+ (firstn (Log.addr_count rec2 + Log.data_count rec2)
+    (skipn (Log.start rec2) log2))))
+(ATCD_reboot_list n).
+Proof.
+ Transparent Log.apply_txn.
+ unfold Log.apply_txn, apply_txn_precondition; simpl; intros.
+ logic_clean.
+ simpl; eapply ATCD_TS_compositional; 
+ simpl; intros; eauto.
+ 
+ eapply ATCD_TS_Log_decrypt_txn; eauto.
+ {
+    repeat invert_lift2.
+    unfold equivalent_for_recovery in *; logic_clean.
+    eapply Specs.decrypt_txn_finished in H14; eauto.
+    eapply Specs.decrypt_txn_finished in H20; eauto.
+
+    eapply TS_eqv_impl.
+    eapply ATCD_TS_BatchOperations_write_batch; eauto.
+    all: try solve [logic_clean; subst; simpl in *; eauto].
+    instantiate (5:= fun _ _ s0 s3 => equivalent_for_recovery txns1 txns2 Log.Current_Part hdr1 hdr2 s0 s3).
+    simpl; eauto.
+ }
+ {
+    simpl.
+    repeat invert_lift2.
+    unfold equivalent_for_recovery in *; logic_clean.
+    eapply Specs.decrypt_txn_finished in H14; eauto.
+    eapply Specs.decrypt_txn_finished in H20; eauto.
+    cleanup.
+    repeat cleanup_pairs; simpl in *.
+    eexists (_, (_, _)), (_, (_, _));
+    simpl; intuition eauto.
+    do 2 eexists; intuition eauto; try congruence.
+    eapply RepImplications.log_rep_explicit_consistent_with_upds; eauto.
+    do 2 eexists; intuition eauto; try congruence.
+    eapply RepImplications.log_rep_explicit_consistent_with_upds; eauto.
+ }
 Qed.
 
 
-Lemma Log_TS_decrypt_txns:
-forall u records1 records2 s1 s2 o s1' t log1 log2,
+Definition record0 := Log.Build_txn_record key0 0 0 0.
 
-exec (CryptoDiskLang) u o s1 
-(decrypt_txns records1 log1)
-     (Finished s1' t) ->
+Fixpoint consistent_with_upds_list {A AEQ V} (m: @mem A AEQ V) l_l_a l_l_v :=
+ match l_l_a, l_l_v with
+ |l_a :: l_l_a', l_v :: l_l_v' =>
+    consistent_with_upds m l_a l_v /\
+    consistent_with_upds_list (Mem.upd_batch m l_a l_v) l_l_a' l_l_v'
+ |_, _ => True
+ end.
 
-length records1 = length records2 ->
-
-Forall2 (fun a t => length (firstn (addr_count a + data_count a) (skipn (start a) log1)) =
-length (firstn (addr_count t + data_count t) (skipn (start t) log2))) records1 records2 ->
-
-Forall (fun record2 => Forall2 (fun a v => (snd (fst s2)) a = Some v)
-(firstn (addr_count record2 + data_count record2)
-(skipn (start record2) log2))
-(map (fun ev : value => (key record2, decrypt (key record2) ev))
-(firstn (addr_count record2 + data_count record2)
-   (skipn (start record2) log2)))) records2 ->
-
-Forall (fun t => length (firstn (data_count t) (blocks_to_addr_list (firstn (addr_count t) (map (decrypt (key t)) (firstn (addr_count t + data_count t) (skipn (start t) log2)))))) =
-length (skipn (addr_count t) (map (decrypt (key t)) (firstn (addr_count t + data_count t) (skipn (start t) log2))))) records2 ->
-
-exists s2' t,
-exec (CryptoDiskLang) u o s2 (decrypt_txns records2 log2) (Finished s2' t).
+Lemma ATCD_TS_Log_apply_txns:
+forall recs1 log1 recs2 log2 n u txns1 txns2 hdr1 hdr2,
+length recs1 = length recs2 ->
+ Forall2 (apply_txn_precondition log1 log2) recs1 recs2 ->
+Termination_Sensitive u 
+(@lift_L2 AuthenticationOperation _ TCDLang _
+(@lift_L2 _ _ CachedDiskLang _
+   (|CDDP| Log.apply_txns recs1 log1)))
+(@lift_L2 AuthenticationOperation _ TCDLang _
+   (@lift_L2 _ _ CachedDiskLang _
+      (|CDDP| Log.apply_txns recs2 log2)))
+ (Simulation.Definitions.compile
+   ATCD_Refinement
+   (Simulation.Definitions.compile
+ ATC_Refinement
+ (Simulation.Definitions.compile
+    FD.refinement
+    (| Recover |))))
+(refines_valid ATCD_Refinement
+(refines_valid ATC_Refinement AD_valid_state)) 
+(fun s1 s2 => equivalent_for_recovery txns1 txns2 Log.Current_Part hdr1 hdr2 s1 s2 /\
+(consistent_with_upds_list (snd (fst (snd (snd (snd s2))))) 
+(map (fun rec2 => (firstn (Log.addr_count rec2 + Log.data_count rec2)
+(skipn (Log.start rec2) log2))) recs2)
+(map (fun rec2 => (map 
+(fun ev : value => (Log.key rec2, decrypt (Log.key rec2) ev))
+(firstn (Log.addr_count rec2 + Log.data_count rec2)
+   (skipn (Log.start rec2) log2)))) recs2)))
+(ATCD_reboot_list n).
 Proof.
-     induction records1; 
-     destruct records2; simpl; intros; 
-     try lia;repeat invert_exec.
-     repeat econstructor.
-     inversion H1; inversion H2; inversion H3; cleanup.
-     eapply Log_TS_decrypt_txn with (s2:= s2) (record2:= t) (log2:= log2) in H; cleanup.
-     eapply IHrecords1 in H4; cleanup.
+ Transparent Log.apply_txns.
+ Opaque Log.apply_txn.
+ induction recs1; destruct recs2; simpl; 
+ intros; try lia.
+ eapply TS_eqv_impl.
+ apply ATCD_TS_ret.
+ intuition eauto.
 
-     do 2 eexists; repeat econstructor; eauto.
-     all: eauto.
-     {
-          eapply decrypt_txn_finished in H; cleanup.
-          eapply Forall_forall; intros.
-          eapply Forall_forall in H14; eauto.
-          eapply forall2_impl; eauto.
-          eapply forall_forall2.
-          rewrite combine_map_r.
-          eapply Forall_forall; intros.
-          apply in_map_iff in H11; cleanup; simpl in *.
-          apply in_combine_same in H15; cleanup.
-          eapply upd_batch_consistent_some in H12; eauto.
-          eapply FunctionalExtensionality.equal_f in H6.
-          rewrite H6; eauto.
+ simpl; eapply ATCD_TS_compositional; 
+ simpl; intros; eauto.
+ 2: eapply IHrecs1; eauto.
+ eapply TS_eqv_impl.
+ eapply ATCD_TS_Log_apply_txn.
+ inversion H0; eauto.
+ intuition eauto.
+ inversion H0; eauto.
 
-          rewrite map_length; eauto.
-          eauto.
-     }
-     eapply in_map_consistent_with_upds; eauto.
-Qed.
-
-Lemma Log_TS_recover:
-forall u s1 s2 o s1' t hdr1 hdr2 txns1 txns2 
-valid_part hdr_blockset1 hdr_blockset2 
-log_blocksets1 log_blocksets2,
-
-exec (CryptoDiskLang) u o s1 Log.recover
-     (Finished s1' t) ->
-
-
-log_rep_explicit Log.Hdr_Synced Log.Synced valid_part hdr1 txns1
-hdr_blockset1 log_blocksets1 s1 -> 
-log_rep_explicit Log.Hdr_Synced Log.Synced valid_part hdr2 txns2
-hdr_blockset2 log_blocksets2 s2 -> 
-
-(valid_part = Log.Old_Part ->
-Log.hash (Log.current_part hdr1) <>
-rolling_hash hash0
-     (firstn (Log.count (Log.current_part hdr1)) (map fst log_blocksets1))) ->
-
-(valid_part = Log.Old_Part ->
-     Log.hash (Log.current_part hdr2) <>
-     rolling_hash hash0
-          (firstn (Log.count (Log.current_part hdr2)) (map fst log_blocksets2))) ->
-
-(valid_part = Old_Part -> count (current_part hdr1) = count (current_part hdr2)) ->
-
-Forall2
-  (fun rec1 rec2 => 
-  start rec1 = start rec2 /\
-  addr_count rec1 = addr_count rec2 /\
-  data_count rec1 = data_count rec2)
-  (map record txns1) (map record txns2) ->
-
-exists s2' t,
-exec (CryptoDiskLang) u o s2 Log.recover
-     (Finished s2' t).
-Proof.
-Transparent Log.recover.
-unfold Log.recover in *.
-simpl in *; intros;
-cleanup; repeat invert_exec.
-eapply_fresh Log_TS_read_encrypted_log in H; eauto; cleanup.
-eapply_fresh Log_TS_write_header in H6; cleanup.
-
-unfold log_header_rep, log_rep_general in *; cleanup.
-eapply read_encrypted_log_finished in H; eauto; intros; try congruence.
-eapply_fresh read_encrypted_log_finished in H7; eauto; intros; try congruence.
-simpl in *; cleanup_no_match; simpl in *.
-
-eapply Log_TS_decrypt_txns in H8; cleanup_no_match.
-do 2 eexists; repeat econstructor; eauto.
-rewrite cons_app.
-repeat econstructor; eauto.
-
+ repeat invert_lift2; cleanup.
+ inversion H0; eauto; cleanup.
+ unfold apply_txn_precondition in H13; logic_clean.
+ eapply Specs.apply_txn_finished in H11; eauto.
+ eapply Specs.apply_txn_finished in H17; eauto.
+ cleanup; repeat cleanup_pairs.
+ simpl in *; intros; intuition eauto.
+ admit.
+ repeat rewrite map_map; simpl.
+ rewrite map_ext at 1.
+ rewrite map_id; eauto.
+ simpl; intros; apply decrypt_encrypt.
 Admitted.
-(* cleanup; eapply forall2_length; eauto. 
-all: simpl; eauto.
-2: {
-     eapply forall2_impl; eauto.
-     eapply forall_forall2.
-     eapply Forall_forall; intros; cleanup; eauto.
-     repeat rewrite firstn_length_l; eauto.
-     
-     rewrite skipn_length.
-     destruct x2; eapply in_combine_r in H; simpl in *.
-     unfold log_rep_explicit, log_rep_inner, txns_valid in *; cleanup.
-     rewrite <- H28 in *; clear H28.
-     apply in_map_iff in H; cleanup; simpl in *.
-     eapply Forall_forall in H29; eauto.
-     unfold txn_well_formed, record_is_valid in H29; cleanup.
-     rewrite firstn_length_l.
-     lia.
-     rewrite map_length; eauto.
-     setoid_rewrite H24; eauto.
 
-     rewrite skipn_length.
-     destruct x2; eapply in_combine_l in H; simpl in *.
-     unfold log_rep_explicit, log_rep_inner, txns_valid in *; cleanup.
-     rewrite <- H36 in *; clear H36.
-     apply in_map_iff in H; cleanup; simpl in *.
-     eapply Forall_forall in H37; eauto.
-     unfold txn_well_formed, record_is_valid in H37; cleanup.
-     rewrite firstn_length_l.
-     lia.
-     rewrite map_length; eauto.
-     setoid_rewrite H32; eauto.
-     eapply forall2_length; eauto.
-}
-{
-     unfold write_header in *; repeat invert_exec.
-     repeat cleanup_pairs; cleanup.
-     eapply Forall_forall; intros; cleanup; eauto.
-     unfold log_rep_explicit, log_rep_inner, txns_valid in *; cleanup.
-     rewrite <- H16 in *; clear H16.
-     apply in_map_iff in H; cleanup; simpl in *.
-     eapply Forall_forall in H17; eauto.
-     unfold txn_well_formed, record_is_valid in H17; cleanup.
-     eapply forall_forall2.
-     rewrite combine_map_r.
-     eapply Forall_forall; intros.
-     apply in_map_iff in H34; cleanup; simpl in *.
-     apply in_combine_same in H35; cleanup.
-     rewrite <- skipn_firstn_comm in H34.
-     rewrite firstn_firstn in H34.
-     rewrite min_l in H34 by lia.
-     rewrite skipn_firstn_comm in H34.
-     rewrite firstn_sum_split in H34.
-     apply in_app_iff in H34.
-     split_ors.
+Lemma ATCD_TS_Log_flush_txns:
+forall n u recs1 recs2 log1 log2 txns1 txns2 hdr1 hdr2,
+length recs1 = length recs2 ->
+ Forall2 (apply_txn_precondition log1 log2) recs1 recs2 ->
 
-     rewrite <- H1 in H34.
-     apply in_map_iff in H34; cleanup.
-     eapply in_seln_exists in H36; cleanup.
-     rewrite <- H34, <- H37; eauto.
-     rewrite encrypt_decrypt.
-     apply H31; eauto.
-     
-     rewrite skipn_skipn in H34.
-     rewrite <- H12 in H34.
-     apply in_map_iff in H34; cleanup.
-     eapply in_seln_exists in H36; cleanup.
-     rewrite <- H34, <- H37; eauto.
-     rewrite encrypt_decrypt.
-     apply H32; eauto.
-     rewrite map_length; eauto.
-}
-{
-     repeat cleanup_pairs; cleanup.
-     eapply Forall_forall; intros; cleanup; eauto.
-     unfold log_rep_explicit, log_rep_inner, txns_valid in *; cleanup.
-     rewrite <- H19 in *; clear H19.
-     apply in_map_iff in H; cleanup; simpl in *.
-     eapply Forall_forall in H20; eauto.
-     unfold txn_well_formed, record_is_valid in H20; cleanup.
-     rewrite firstn_length_l.
-     rewrite skipn_length, map_length.
-     rewrite firstn_length_l.
-     lia.
-     rewrite skipn_length.
-     rewrite firstn_length_l.
-     lia.
-     rewrite map_length. 
-     setoid_rewrite H13; eauto.
-
-     eapply PeanoNat.Nat.le_trans.
-     eauto.
-     apply blocks_to_addr_list_length_le_preserve.
-     rewrite firstn_length_l; eauto.
-     rewrite map_length.
-     rewrite firstn_length_l.
-     lia.
-     rewrite skipn_length.
-     rewrite firstn_length_l.
-     lia.
-     rewrite map_length. 
-     setoid_rewrite H13; eauto.
-}
-Qed.
-*)
-
-
-
-
-
-(***** Crashed TS *****)
-Lemma Log_TS_read_header_crashed:
-forall u s1 s2 o s1' ,
-exec (CryptoDiskLang) u o s1 read_header (Crashed s1') ->
-exists s2',
-exec (CryptoDiskLang) u o s2 read_header (Crashed s2').
+Termination_Sensitive u 
+(@lift_L2 AuthenticationOperation _ TCDLang _
+(@lift_L2 _ _ CachedDiskLang _
+   (|CDDP| Log.flush_txns recs1 log1)))
+(@lift_L2 AuthenticationOperation _ TCDLang _
+   (@lift_L2 _ _ CachedDiskLang _
+      (|CDDP| Log.flush_txns recs2 log2)))
+ (Simulation.Definitions.compile
+   ATCD_Refinement
+   (Simulation.Definitions.compile
+ ATC_Refinement
+ (Simulation.Definitions.compile
+    FD.refinement
+    (| Recover |))))
+(refines_valid ATCD_Refinement
+(refines_valid ATC_Refinement AD_valid_state)) 
+(fun s1 s2 => equivalent_for_recovery txns1 txns2 Log.Current_Part hdr1 hdr2 s1 s2 /\
+(consistent_with_upds_list (snd (fst (snd (snd (snd s2))))) 
+(map (fun rec2 => (firstn (Log.addr_count rec2 + Log.data_count rec2)
+(skipn (Log.start rec2) log2))) recs2)
+(map (fun rec2 => (map 
+(fun ev : value => (Log.key rec2, decrypt (Log.key rec2) ev))
+(firstn (Log.addr_count rec2 + Log.data_count rec2)
+   (skipn (Log.start rec2) log2)))) recs2)))
+(ATCD_reboot_list n).
 Proof.
-unfold read_header in *.
-simpl in *; intros;
-cleanup; repeat invert_exec.
-split_ors; cleanup; repeat invert_exec.
-eexists; repeat econstructor; eauto.
-eexists; repeat econstructor; eauto.
-Qed.
+ unfold Log.flush_txns.
+ intros; simpl.
+ eapply ATCD_TS_compositional.
+ intros; apply ATCD_TS_Log_apply_txns; eauto.
+ simpl; intros.
+ 
+ eapply ATCD_TS_compositional.
+ intros; eapply ATCD_TS_Disk_sync.
 
-
-Lemma Log_TS_write_header_crashed:
-forall u s1 s2 o s1' hdr1 hdr2,
-exec (CryptoDiskLang) u o s1 
-(write_header hdr1) (Crashed s1') ->
-exists s2',
-exec (CryptoDiskLang) u o s2 
-(write_header hdr2) (Crashed s2').
-Proof.
-unfold write_header in *.
-simpl in *; intros;
-cleanup; repeat invert_exec.
-eexists; repeat econstructor; eauto.
-Qed.
-
-
-
-Lemma Log_TS_check_hash_crashed:
-forall u l1 l2 s1 s2 o s1' h1 h2,
-exec (CryptoDiskLang) u o s1 
-(check_hash l1 h1)
-     (Crashed s1') ->
-     length l1 = length l2 ->
-consistent_with_upds (snd (fst (fst s2))) (rolling_hash_list hash0 l2)
-(combine (hash0 :: rolling_hash_list hash0 l2) l2) ->
-exists s2',
-exec (CryptoDiskLang) u o s2 
-(check_hash l2 h2)
-     (Crashed s2').
-Proof.
-unfold check_hash in *.
-simpl in *; intros;
-cleanup_no_match; repeat invert_exec_no_match.
-split_ors; cleanup_no_match.
-eapply BatchOperations_TS_hash_all_crashed with 
-(s2 := s2) (l2:= l2)in H; cleanup_no_match.
-eexists; repeat econstructor; eauto.
-all: eauto.
-
-eapply BatchOperations_TS_hash_all with 
-(s2 := s2) (l2:= l2)in H2; cleanup_no_match.
-destruct (hash_dec x0 h1);
-repeat invert_exec_no_match;
-destruct (hash_dec x4 h2);
-eexists; repeat econstructor; eauto;
-destruct (hash_dec x4 h2); try congruence; try econstructor.
-all: eauto.
-Qed.
-
-
-Lemma Log_TS_read_encrypted_log_crashed:
-forall u s1 s2 o s1' hdr1 hdr2 txns1 txns2
-valid_part hdr_blockset1 hdr_blockset2 
-log_blocksets1 log_blocksets2,
-
-exec (CryptoDiskLang) u o s1 read_encrypted_log (Crashed s1') ->
-
-log_rep_explicit Log.Hdr_Synced Log.Synced valid_part hdr1 txns1
-hdr_blockset1 log_blocksets1 s1 -> 
-log_rep_explicit Log.Hdr_Synced Log.Synced valid_part hdr2 txns2
-hdr_blockset2 log_blocksets2 s2 -> 
-
-(Log.hash (Log.current_part hdr1) <>
-rolling_hash hash0
-     (firstn (Log.count (Log.current_part hdr1)) (map fst log_blocksets1)) <->
-Log.hash (Log.current_part hdr2) <>
-     rolling_hash hash0
-          (firstn (Log.count (Log.current_part hdr2)) (map fst log_blocksets2))) ->
-
-Forall2
-(fun rec1 rec2 : Log.txn_record =>
-     Log.start rec1 = Log.start rec2 /\
-     Log.addr_count rec1 = Log.addr_count rec2 /\
-     Log.data_count rec1 = Log.data_count rec2)
-(map Log.record txns1)
-(map Log.record txns2) ->
-
-consistent_with_upds (snd (fst (fst s2)))
-  (rolling_hash_list hash0
-     (firstn (count (current_part hdr2)) (map fst log_blocksets2)))
-  (combine
-     (hash0
-      :: rolling_hash_list hash0
-           (firstn (count (current_part hdr2)) (map fst log_blocksets2)))
-     (firstn (count (current_part hdr2)) (map fst log_blocksets2))) ->
-
-consistent_with_upds (snd (fst (fst s2)))
-  (rolling_hash_list hash0
-     (firstn (count (old_part hdr2)) (map fst log_blocksets2)))
-  (combine
-     (hash0
-      :: rolling_hash_list hash0
-           (firstn (count (old_part hdr2)) (map fst log_blocksets2)))
-     (firstn (count (old_part hdr2)) (map fst log_blocksets2))) ->
-
-(valid_part = Old_Part -> count (current_part hdr1) = count (current_part hdr2)) ->
-
-exists s2',
-exec (CryptoDiskLang) u o s2 read_encrypted_log (Crashed s2').
-Proof.
-Opaque read_header check_hash.
-unfold read_encrypted_log in *.
-simpl in *; intros;
-cleanup_no_match; repeat invert_exec_no_match.
-split_ors; cleanup_no_match; repeat invert_exec_no_match.
-{
-     eapply_fresh Log_TS_read_header_crashed with (s2:= s2) in H; cleanup_no_match.
-     eexists; repeat econstructor; eauto.
-}
-
-eapply_fresh Log_TS_read_header with (s2:= s2) in H7; cleanup_no_match.
-eapply_fresh Log_read_header_finished in H; eauto.
-eapply_fresh Log_read_header_finished in H7; eauto.
-cleanup_no_match.
-assume (A: (count (current_part hdr1) = count (current_part hdr2))).
-split_ors; cleanup_no_match; repeat invert_exec_no_match.
-{
-     eapply_fresh BatchOperations_TS_read_consecutive_crashed with (s2:= s2) in H8; cleanup_no_match.
-     eexists; repeat econstructor; eauto.
-
-     pose proof data_fits_in_disk.
-     pose proof data_start_where_log_ends.
-     pose proof all_fits_to_data_region.
-     unfold log_header_rep, log_rep_general,  log_rep_explicit in *; logic_clean.
-     lia.
-}
-
-eapply_fresh BatchOperations_TS_read_consecutive with (s2:= s2) in H9; cleanup_no_match.
-unfold log_header_rep, log_rep_general in *; cleanup_no_match.
-eapply_fresh Log_read_log in H9; eauto.
-eapply_fresh Log_read_log in H8; eauto.
-2: eauto.
-cleanup_no_match.
-
-split_ors; cleanup_no_match; repeat invert_exec_no_match.
-{
-     eapply_fresh Log_TS_check_hash_crashed with (s2 := s2) in H10; cleanup_no_match.
-     eexists; repeat econstructor; eauto.
-     repeat rewrite firstn_length_l; eauto.
-
-     rewrite map_length.
-     unfold  log_rep_explicit in *; logic_clean.
-     setoid_rewrite H13; eauto.
-
-     rewrite map_length.
-     unfold  log_rep_explicit in *; logic_clean.
-     setoid_rewrite H19; eauto.
-
-     eauto.
-}
-
-eapply_fresh Log_TS_check_hash with (s2 := s2) in H11; cleanup_no_match.
-
-eapply_fresh Log_check_hash_finished in H11; eauto; cleanup_no_match.
-eapply_fresh Log_check_hash_finished in H10; eauto; cleanup_no_match.
-repeat split_ors; logic_clean; subst; try congruence.
-{
-     eexists; repeat econstructor; eauto.
-     simpl; repeat invert_exec_no_match; repeat econstructor.
-}
-{
-     exfalso; destruct H2; apply H2; eauto.
-}
-{
-     exfalso; apply H2; eauto.
-}
-
-repeat invert_exec_no_match.
-assume (A0: (count (old_part hdr1) = count (old_part hdr2))).
-split_ors; cleanup_no_match; repeat invert_exec_no_match.
-{
-     eapply_fresh BatchOperations_TS_read_consecutive_crashed with (s2:= x4) in H12; cleanup_no_match.
-     eexists; repeat econstructor; eauto.
-     simpl; repeat econstructor; eauto.
-
-     pose proof data_fits_in_disk.
-     pose proof data_start_where_log_ends.
-     pose proof all_fits_to_data_region.
-     unfold log_header_rep, log_rep_general,  log_rep_explicit in *; logic_clean.
-     lia.
-}
-{
-     eapply_fresh BatchOperations_TS_read_consecutive with (s2:= x4) in H13; cleanup_no_match.
-     eexists; repeat econstructor; eauto.
-     simpl; repeat econstructor; eauto.
-
-     pose proof data_fits_in_disk.
-     pose proof data_start_where_log_ends.
-     pose proof all_fits_to_data_region.
-     unfold log_header_rep, log_rep_general,  log_rep_explicit in *; logic_clean.
-     lia.
-}
-
-repeat rewrite firstn_length_l; eauto.
-rewrite map_length.
-unfold  log_rep_explicit in *; logic_clean.
-setoid_rewrite H14; eauto.
-
-rewrite map_length.
-unfold  log_rep_explicit in *; logic_clean.
-setoid_rewrite H20; eauto.
-
-eauto.
-
-pose proof data_fits_in_disk.
-pose proof data_start_where_log_ends.
-pose proof all_fits_to_data_region.
-unfold log_header_rep, log_rep_general,  log_rep_explicit in *; logic_clean.
-lia.
-
-pose proof data_fits_in_disk.
-pose proof data_start_where_log_ends.
-pose proof all_fits_to_data_region.
-unfold log_header_rep, log_rep_general,  log_rep_explicit in *; logic_clean.
-lia.
-
-pose proof data_fits_in_disk.
-pose proof data_start_where_log_ends.
-pose proof all_fits_to_data_region.
-unfold log_header_rep, log_rep_general,  log_rep_explicit in *; logic_clean.
-lia.
-
-Unshelve.
-all: admit.
+ simpl; intros.
+ eapply ATCD_TS_compositional.
+ intros; eapply ATCD_TS_Log_update_header.
+ intros; eapply ATCD_TS_Disk_sync.
+ 
+ all: admit. (* Make lemmas *)
+ Opaque Log.flush_txns.
 Admitted.
 
 
-
-Lemma Log_TS_decrypt_txn_crashed:
-forall u record1 record2 s1 s2 o s1' log1 log2,
-
-exec (CryptoDiskLang) u o s1 
-(decrypt_txn record1 log1)
-     (Crashed s1') ->
-
-length
-     (firstn (addr_count record1 + data_count record1)
-        (skipn (start record1) log1)) =
-length
-     (firstn (addr_count record2 + data_count record2)
-        (skipn (start record2) log2)) ->
-   
-consistent_with_upds (snd (fst s2))
-     (firstn (addr_count record2 + data_count record2)
-        (skipn (start record2) log2))
-     (map (fun ev : value => (key record2, decrypt (key record2) ev))
-        (firstn (addr_count record2 + data_count record2)
-           (skipn (start record2) log2))) ->
-
-exists s2',
-exec (CryptoDiskLang) u o s2 (decrypt_txn record2 log2) (Crashed s2').
+Lemma ATCD_TS_Log_apply_log:
+forall n u txns1 txns2 hdr1 hdr2,
+Termination_Sensitive u 
+(@lift_L2 AuthenticationOperation _ TCDLang _
+(@lift_L2 _ _ CachedDiskLang _
+   (|CDDP| Log.apply_log)))
+(@lift_L2 AuthenticationOperation _ TCDLang _
+   (@lift_L2 _ _ CachedDiskLang _
+      (|CDDP| Log.apply_log)))
+ (Simulation.Definitions.compile
+   ATCD_Refinement
+   (Simulation.Definitions.compile
+ ATC_Refinement
+ (Simulation.Definitions.compile
+    FD.refinement
+    (| Recover |))))
+(refines_valid ATCD_Refinement
+(refines_valid ATC_Refinement AD_valid_state)) 
+(equivalent_for_recovery txns1 txns2 Log.Current_Part hdr1 hdr2)
+(ATCD_reboot_list n).
 Proof.
-     unfold decrypt_txn; intros; repeat invert_exec.
-     split_ors; cleanup; repeat invert_exec.
-     {
-          eapply BatchOperations_TS_decrypt_all_crashed in H; eauto.
-          cleanup.
-          eexists; repeat constructor; eauto.
-     }
-
-     eapply BatchOperations_TS_decrypt_all with (s2:= s2) (k2:= (key record2)) 
-     (l2 := firstn (addr_count record2 + data_count record2)
-     (skipn (start record2) log2)) in H2; cleanup.
-     eexists; repeat econstructor; eauto.
-     all: eauto.
-Qed.
-
-
-Lemma Log_TS_decrypt_txns_crashed:
-forall u records1 records2 s1 s2 o s1' log1 log2,
-
-exec (CryptoDiskLang) u o s1 
-(decrypt_txns records1 log1)
-     (Crashed s1') ->
-
-length records1 = length records2 ->
-
-Forall2 (fun a t => length (firstn (addr_count a + data_count a) (skipn (start a) log1)) =
-length (firstn (addr_count t + data_count t) (skipn (start t) log2))) records1 records2 ->
-
-Forall (fun record2 => Forall2 (fun a v => (snd (fst s2)) a = Some v)
-(firstn (addr_count record2 + data_count record2)
-(skipn (start record2) log2))
-(map (fun ev : value => (key record2, decrypt (key record2) ev))
-(firstn (addr_count record2 + data_count record2)
-   (skipn (start record2) log2)))) records2 ->
-
-Forall (fun t => length (firstn (data_count t) (blocks_to_addr_list (firstn (addr_count t) (map (decrypt (key t)) (firstn (addr_count t + data_count t) (skipn (start t) log2)))))) =
-length (skipn (addr_count t) (map (decrypt (key t)) (firstn (addr_count t + data_count t) (skipn (start t) log2))))) records2 ->
-
-exists s2',
-exec (CryptoDiskLang) u o s2 (decrypt_txns records2 log2) (Crashed s2').
-Proof.
-     induction records1; 
-     destruct records2; simpl; intros; 
-     try lia;repeat invert_exec.
-     repeat econstructor.
-
-     inversion H1; inversion H2; inversion H3; cleanup.
-     split_ors; cleanup; repeat invert_exec.
-     {
-          eapply Log_TS_decrypt_txn_crashed with (s2:= s2) (record2:= t) (log2:= log2) in H; cleanup.
-          eexists; econstructor; eauto.
-          all: eauto.
-          eapply in_map_consistent_with_upds; eauto.
-     }
-eapply Log_TS_decrypt_txn with (s2:= s2) (record2:= t) (log2:= log2) in H4; cleanup.
-split_ors; cleanup; repeat invert_exec.
-{
-     eapply IHrecords1 in H4; cleanup.
-
-     eexists; repeat econstructor; eauto.
-     all: eauto.
-     {
-          eapply decrypt_txn_finished in H; cleanup.
-          eapply Forall_forall; intros.
-          eapply Forall_forall in H13; eauto.
-          eapply forall2_impl; eauto.
-          eapply forall_forall2.
-          rewrite combine_map_r.
-          eapply Forall_forall; intros.
-          apply in_map_iff in H11; cleanup; simpl in *.
-          apply in_combine_same in H15; cleanup.
-          eapply upd_batch_consistent_some in H10; eauto.
-          eapply FunctionalExtensionality.equal_f in H6.
-          rewrite H6; eauto.
-
-          rewrite map_length; eauto.
-          eauto.
-     }
-}
-{
-     eapply Log_TS_decrypt_txns in H5; cleanup.
-     eexists; repeat econstructor; eauto.
-     all: eauto.
-     {
-          eapply decrypt_txn_finished in H; cleanup.
-          eapply Forall_forall; intros.
-          eapply Forall_forall in H13; eauto.
-          eapply forall2_impl; eauto.
-          eapply forall_forall2.
-          rewrite combine_map_r.
-          eapply Forall_forall; intros.
-          apply in_map_iff in H11; cleanup; simpl in *.
-          apply in_combine_same in H15; cleanup.
-          eapply upd_batch_consistent_some in H10; eauto.
-          eapply FunctionalExtensionality.equal_f in H6.
-          rewrite H6; eauto.
-
-          rewrite map_length; eauto.
-          eauto.
-     }
-}
-all: eauto.
-eapply in_map_consistent_with_upds; eauto.
-Qed.
-
-Lemma Log_TS_recover_crashed:
-forall u s1 s2 o s1' hdr1 hdr2 txns1 txns2 
-valid_part hdr_blockset1 hdr_blockset2 
-log_blocksets1 log_blocksets2,
-
-exec (CryptoDiskLang) u o s1 Log.recover (Crashed s1') ->
-
-
-log_rep_explicit Log.Hdr_Synced Log.Synced valid_part hdr1 txns1
-hdr_blockset1 log_blocksets1 s1 -> 
-log_rep_explicit Log.Hdr_Synced Log.Synced valid_part hdr2 txns2
-hdr_blockset2 log_blocksets2 s2 -> 
-
-(valid_part = Log.Old_Part ->
-Log.hash (Log.current_part hdr1) <>
-rolling_hash hash0
-     (firstn (Log.count (Log.current_part hdr1)) (map fst log_blocksets1))) ->
-
-(valid_part = Log.Old_Part ->
-     Log.hash (Log.current_part hdr2) <>
-     rolling_hash hash0
-          (firstn (Log.count (Log.current_part hdr2)) (map fst log_blocksets2))) ->
-
-(valid_part = Old_Part -> count (current_part hdr1) = count (current_part hdr2)) ->
-
-Forall2
-  (fun rec1 rec2 => 
-  start rec1 = start rec2 /\
-  addr_count rec1 = addr_count rec2 /\
-  data_count rec1 = data_count rec2)
-  (map record txns1) (map record txns2) ->
-
-exists s2',
-exec (CryptoDiskLang) u o s2 Log.recover (Crashed s2').
-Proof.
-Opaque Log.read_encrypted_log.
-Transparent Log.recover.
-unfold Log.recover in *.
-simpl in *; intros;
-cleanup; repeat invert_exec.
-split_ors; cleanup_no_match; repeat invert_exec_no_match.
-{
-     eapply_fresh Log_TS_read_encrypted_log_crashed in H; eauto; cleanup.
-     eexists; repeat econstructor; eauto.
-     all: eauto.
-     all: admit.
-}
-eapply_fresh Log_TS_read_encrypted_log in H6; eauto; cleanup.
-unfold log_header_rep, log_rep_general in *; cleanup.
-eapply_fresh read_encrypted_log_finished in H; eauto; intros; try congruence.
-eapply_fresh read_encrypted_log_finished in H6; eauto; intros; try congruence.
-simpl in *; cleanup_no_match; simpl in *.
-
-split_ors; cleanup_no_match; repeat invert_exec_no_match.
-{
-     eapply_fresh Log_TS_write_header_crashed in H7; cleanup_no_match.
-     eexists; repeat econstructor; eauto.
-}
-eapply_fresh Log_TS_write_header in H8; cleanup_no_match.
-split_ors; cleanup_no_match; repeat invert_exec_no_match.
-{
-     eexists; repeat econstructor; eauto.
-}
-(*
-unfold log_header_rep, log_rep_general in *; cleanup.
-eapply read_encrypted_log_finished in H; eauto; intros; try congruence.
-eapply_fresh read_encrypted_log_finished in H7; eauto; intros; try congruence.
-simpl in *; cleanup_no_match; simpl in *.
-*)
-eapply Log_TS_decrypt_txns_crashed in e1; cleanup_no_match.
-eexists; repeat econstructor; eauto.
-all: simpl; eauto.
-
+ Transparent Log.apply_log.
+ unfold Log.apply_log; intros.
+ simpl. eapply ATCD_TS_compositional.
+ intros; apply ATCD_TS_Log_read_encrypted_log.
+ 
+ intros; cleanup; eauto.
+ repeat invert_lift2; cleanup.
+ unfold equivalent_for_recovery in *; logic_clean.
+ eapply Specs.read_encrypted_log_finished in H7; eauto.
+ eapply Specs.read_encrypted_log_finished in H13; eauto.
+ simpl in *; cleanup; simpl in *.
+ eapply TS_eqv_impl.
+ eapply ATCD_TS_Log_flush_txns; eauto.
+ shelve.
+ shelve.
+ shelve.
+ shelve.
+ Opaque Log.apply_log.
 Admitted.
-(* cleanup; eapply forall2_length; eauto. 
-all: simpl; eauto.
-2: {
-     eapply forall2_impl; eauto.
-     eapply forall_forall2.
-     eapply Forall_forall; intros; cleanup; eauto.
-     repeat rewrite firstn_length_l; eauto.
-     
-     rewrite skipn_length.
-     destruct x2; eapply in_combine_r in H; simpl in *.
-     unfold log_rep_explicit, log_rep_inner, txns_valid in *; cleanup.
-     rewrite <- H28 in *; clear H28.
-     apply in_map_iff in H; cleanup; simpl in *.
-     eapply Forall_forall in H29; eauto.
-     unfold txn_well_formed, record_is_valid in H29; cleanup.
-     rewrite firstn_length_l.
-     lia.
-     rewrite map_length; eauto.
-     setoid_rewrite H24; eauto.
 
-     rewrite skipn_length.
-     destruct x2; eapply in_combine_l in H; simpl in *.
-     unfold log_rep_explicit, log_rep_inner, txns_valid in *; cleanup.
-     rewrite <- H36 in *; clear H36.
-     apply in_map_iff in H; cleanup; simpl in *.
-     eapply Forall_forall in H37; eauto.
-     unfold txn_well_formed, record_is_valid in H37; cleanup.
-     rewrite firstn_length_l.
-     lia.
-     rewrite map_length; eauto.
-     setoid_rewrite H32; eauto.
-     eapply forall2_length; eauto.
-}
-{
-     unfold write_header in *; repeat invert_exec.
-     repeat cleanup_pairs; cleanup.
-     eapply Forall_forall; intros; cleanup; eauto.
-     unfold log_rep_explicit, log_rep_inner, txns_valid in *; cleanup.
-     rewrite <- H16 in *; clear H16.
-     apply in_map_iff in H; cleanup; simpl in *.
-     eapply Forall_forall in H17; eauto.
-     unfold txn_well_formed, record_is_valid in H17; cleanup.
-     eapply forall_forall2.
-     rewrite combine_map_r.
-     eapply Forall_forall; intros.
-     apply in_map_iff in H34; cleanup; simpl in *.
-     apply in_combine_same in H35; cleanup.
-     rewrite <- skipn_firstn_comm in H34.
-     rewrite firstn_firstn in H34.
-     rewrite min_l in H34 by lia.
-     rewrite skipn_firstn_comm in H34.
-     rewrite firstn_sum_split in H34.
-     apply in_app_iff in H34.
-     split_ors.
+Lemma ATCD_TS_Log_commit:
+forall n u lo s1 s2 l_a1 l_a2 l_v1 l_v2 txns1 txns2 hdr1 hdr2,
+length ((addr_list_to_blocks (map (Nat.add data_start) l_a1)) ++ l_v1) = 
+length ((addr_list_to_blocks (map (Nat.add data_start) l_a2)) ++ l_v2) ->
+(log_length < (Log.count (Log.current_part hdr1) +
+    (length (addr_list_to_blocks (map (Nat.add data_start) l_a1)) + length l_v1)) <-> 
+  log_length < (Log.count (Log.current_part hdr2) +
+    (length (addr_list_to_blocks (map (Nat.add data_start) l_a2)) + length l_v2))) ->
+Termination_Sensitive_explicit u lo s1 s2
+(@lift_L2 AuthenticationOperation _ TCDLang _
+(@lift_L2 _ _ CachedDiskLang _
+   (|CDDP| Log.commit (addr_list_to_blocks (map (Nat.add data_start) l_a1)) l_v1)))
+(@lift_L2 AuthenticationOperation _ TCDLang _
+   (@lift_L2 _ _ CachedDiskLang _
+      (|CDDP| Log.commit (addr_list_to_blocks (map (Nat.add data_start) l_a2)) l_v2)))
+ (Simulation.Definitions.compile
+   ATCD_Refinement
+   (Simulation.Definitions.compile
+ ATC_Refinement
+ (Simulation.Definitions.compile
+    FD.refinement
+    (| Recover |))))
+(refines_valid ATCD_Refinement
+(refines_valid ATC_Refinement AD_valid_state)) 
+(fun s1 s2 => equivalent_for_recovery txns1 txns2 Log.Current_Part hdr1 hdr2 s1 s2 /\
+ equivalent_for_commit (seln lo 0 []) l_a1 l_v1 l_a2 l_v2 s1 s2)
+(ATCD_reboot_list n).
+Proof.
+ Transparent Log.commit.
+ unfold Log.commit; intros; simpl.
+ eapply ATCD_TS_explicit_compositional.
 
-     rewrite <- H1 in H34.
-     apply in_map_iff in H34; cleanup.
-     eapply in_seln_exists in H36; cleanup.
-     rewrite <- H34, <- H37; eauto.
-     rewrite encrypt_decrypt.
-     apply H31; eauto.
-     
-     rewrite skipn_skipn in H34.
-     rewrite <- H12 in H34.
-     apply in_map_iff in H34; cleanup.
-     eapply in_seln_exists in H36; cleanup.
-     rewrite <- H34, <- H37; eauto.
-     rewrite encrypt_decrypt.
-     apply H32; eauto.
-     rewrite map_length; eauto.
-}
-{
-     repeat cleanup_pairs; cleanup.
-     eapply Forall_forall; intros; cleanup; eauto.
-     unfold log_rep_explicit, log_rep_inner, txns_valid in *; cleanup.
-     rewrite <- H19 in *; clear H19.
-     apply in_map_iff in H; cleanup; simpl in *.
-     eapply Forall_forall in H20; eauto.
-     unfold txn_well_formed, record_is_valid in H20; cleanup.
-     rewrite firstn_length_l.
-     rewrite skipn_length, map_length.
-     rewrite firstn_length_l.
-     lia.
-     rewrite skipn_length.
-     rewrite firstn_length_l.
-     lia.
-     rewrite map_length. 
-     setoid_rewrite H13; eauto.
+ intros; eapply TS_explicit_to_TS.
+ intros; eapply TS_eqv_impl.
+ apply ATCD_TS_Log_read_header.
+ intros; cleanup; eauto.
 
-     eapply PeanoNat.Nat.le_trans.
-     eauto.
-     apply blocks_to_addr_list_length_le_preserve.
-     rewrite firstn_length_l; eauto.
-     rewrite map_length.
-     rewrite firstn_length_l.
-     lia.
-     rewrite skipn_length.
-     rewrite firstn_length_l.
-     lia.
-     rewrite map_length. 
-     setoid_rewrite H13; eauto.
-}
+ Transparent Log.read_header.
+ intros; unfold Log.read_header in *; repeat invert_exec.
+ repeat cleanup_pairs; simpl in *.
+ destruct_fresh (PeanoNat.Nat.ltb log_length
+ (Log.count
+    (Log.current_part
+       (Log.decode_header (fst (s6 hdr_block_num)))) +
+  (length
+     (addr_list_to_blocks (map (Nat.add data_start) l_a1)) +
+   length l_v1)));
+ 
+ destruct_fresh (PeanoNat.Nat.ltb log_length
+ (Log.count
+    (Log.current_part
+       (Log.decode_header (fst (s3 hdr_block_num)))) +
+  (length
+     (addr_list_to_blocks (map (Nat.add data_start) l_a2)) +
+   length l_v2)));
+ try eapply_fresh PeanoNat.Nat.ltb_lt in D;
+ try eapply_fresh PeanoNat.Nat.ltb_lt in D0;
+ try eapply_fresh PeanoNat.Nat.ltb_nlt in D;
+ try eapply_fresh PeanoNat.Nat.ltb_nlt in D0;
+ intuition.
+ intros; eapply TS_explicit_to_TS.
+ eapply TS_eqv_impl.
+ apply ATCD_TS_ret.
+ shelve.
+ 
+ unfold equivalent_for_recovery, Log.log_rep_explicit,
+ Log.log_header_block_rep in *; simpl in *; cleanup; lia.
 
-Qed.
-*)
+ unfold equivalent_for_recovery, Log.log_rep_explicit,
+ Log.log_header_block_rep in *; simpl in *; cleanup; lia.
+ 
+ simpl.
+ eapply  ATCD_TS_explicit_compositional.
+ intros; eapply TS_explicit_eqv_impl.
+ intros; eapply ATCD_TS_Log_commit_txn; eauto.
+ 
+ instantiate (1:= Log.decode_header (fst (s3 hdr_block_num))); lia.
+ 
+ simpl; eauto.
+ instantiate (4:= fun _ _ s9 s10 => 
+ equivalent_for_recovery txns1 
+ txns2 Log.Current_Part hdr1 hdr2 s9 s10 /\
+equivalent_for_commit (seln lo 0 []) l_a1 l_v1
+ l_a2 l_v2 s9 s10).
+
+ simpl; intros; simpl in *; cleanup.
+ shelve.
+ 
+ simpl; intros; eapply TS_explicit_to_TS; apply ATCD_TS_ret.
+ simpl.
+ simpl; intros;
+ repeat invert_lift2; cleanup_no_match.
+ simpl in *; cleanup_no_match.
+ (*
+ eapply Specs.commit_txn_finished in H15; eauto.
+ eapply Specs.commit_txn_finished in H22; eauto.
+ cleanup_no_match.
+ repeat cleanup_pairs; simpl in *.
+ *)
+ shelve.
+
+ simpl; intros; unfold Log.read_header in *; repeat invert_exec.
+ repeat cleanup_pairs; simpl in *.
+ eauto.
+
+ Unshelve.
+ 5: simpl; intros; intuition eauto.
+ Opaque Log.commit.
+Admitted.
+ 
+
+ Lemma Log_commit_ret_eq:
+ forall u l_a1 l_v1 l_a2 l_v2 o s1 s2 s1' s2' r1 r2,
+ exec CryptoDisk u o s1 (Log.commit l_a1 l_v1) (Finished s1' r1) ->
+
+ exec CryptoDisk u o s2 (Log.commit l_a2 l_v2) (Finished s2' r2) ->
+ (log_length <
+ (Log.count
+    (Log.current_part (Log.decode_header (fst (snd s1 hdr_block_num)))) +
+  (length l_a1 + length l_v1)) <-> 
+  log_length <
+    (Log.count
+       (Log.current_part (Log.decode_header (fst (snd s2 hdr_block_num)))) +
+     (length l_a2 + length l_v2))) ->
+ r1 = r2.
+ Proof.
+    Transparent Log.commit.
+    unfold Log.commit, Log.read_header.
+    intros; repeat invert_exec; eauto; 
+    repeat cleanup_pairs;
+    try eapply_fresh PeanoNat.Nat.ltb_lt in D;
+    try eapply_fresh PeanoNat.Nat.ltb_lt in D0;
+    try eapply_fresh PeanoNat.Nat.ltb_nlt in D;
+    try eapply_fresh PeanoNat.Nat.ltb_nlt in D0;
+    lia.
+    Opaque Log.commit.
+ Qed.
+
