src/Noninterference/LoggedDisk/TS/ATCD_TS.v
@@ -1,0 +1,6 @@
+Require Export ATCD_TS_Recovery.
+Require Export ATCD_TS_Operations.
+Require Export ATCD_TS_Common.
+Require Export ATCD_TS_Transaction.
+Require Export ATCD_TS_Allocator.
+Require Export ATCD_TS_Inode.
