src/Noninterference/LoggedDisk/TS/ATCD_TS_Allocator.v
@@ -1,0 +1,486 @@
+Require Import Eqdep Lia Framework FSParameters FileDiskLayer. (* LoggedDiskLayer TransactionCacheLayer TransactionalDiskLayer. *)
+Require Import FileDiskNoninterference FileDiskRefinement.
+Require Import ATCDLayer FileDisk.TransferProofs ATCD_Simulation ATCD_AOE.
+Require Import Not_Init HSS ATCD_ORS ATCD_TS_Common ATCD_TS_Recovery ATCD_TS_Transaction.
+
+Import FileDiskLayer.
+Set Nested Proofs Allowed.
+
+Opaque File.recover.
+Lemma ATCD_TS_InodeAllocator_read:
+forall n inum u u' txns1 txns2 hdr1 hdr2,
+Termination_Sensitive u
+(Simulation.Definitions.compile
+ ATCD_Refinement
+ (Simulation.Definitions.compile
+ ATC_Refinement
+(@lift_L2 AuthenticationOperation _ TD _
+    (Inode.InodeAllocator.read inum))))
+(Simulation.Definitions.compile
+ ATCD_Refinement
+ (Simulation.Definitions.compile
+ ATC_Refinement
+(@lift_L2 AuthenticationOperation _ TD _
+    (Inode.InodeAllocator.read inum))))
+(Simulation.Definitions.compile
+ ATCD_Refinement
+ (Simulation.Definitions.compile
+ ATC_Refinement
+ (Simulation.Definitions.compile
+    FD.refinement
+    (| Recover |))))
+(refines_valid ATCD_Refinement
+  (refines_valid ATC_Refinement
+ AD_valid_state))
+(fun s1 s2 => 
+refines_related ATCD_Refinement 
+(fun s1 s2 => refines_related ATC_Refinement
+ (fun s1 s2  => exists s1a s2a, 
+    File.files_inner_rep s1a (fst (snd (snd s1))) /\ 
+    File.files_inner_rep s2a (fst (snd (snd s2))) /\ 
+    FD_related_states u' None s1a s2a) s1 s2 /\
+(forall a, 
+ Transaction.get_first (fst (snd s1)) a = None <-> 
+ Transaction.get_first (fst (snd s2)) a = None)) s1 s2 /\
+ equivalent_for_recovery txns1 txns2 Log.Current_Part hdr1 hdr2 s1 s2 /\
+ (forall a, 
+ fst (snd (snd s1)) a = None <->
+ fst (snd (snd s2)) a = None) /\
+ fst (snd (snd s1)) =
+Mem.list_upd_batch empty_mem
+  (map Log.addr_list txns1)
+  (map Log.data_blocks txns1) /\
+fst (snd (snd s2)) =
+Mem.list_upd_batch empty_mem
+  (map Log.addr_list txns2)
+  (map Log.data_blocks txns2))
+(ATCD_reboot_list n).
+Proof.
+Transparent Inode.InodeAllocator.read.
+unfold Inode.InodeAllocator.read; simpl; intros.
+destruct (Compare_dec.lt_dec inum
+Inode.InodeAllocatorParams.num_of_blocks).
+2: {
+  intros; eapply TS_eqv_impl.
+  apply ATCD_TS_ret.
+  simpl; intuition eauto.
+}
+{
+  eapply ATCD_TS_compositional; simpl.
+  intros; eapply TS_eqv_impl.
+  unfold Inode.InodeAllocatorParams.bitmap_addr in *.
+  pose proof Inode.InodeAllocatorParams.blocks_fit_in_disk.
+  intros; eapply ATCD_TS_Transaction_read.
+  lia.
+  simpl; intros; cleanup; eauto.
+  {
+    intros.
+    unfold refines_related in *; cleanup.
+    simpl in *; unfold HC_refines in *; cleanup.
+    simpl in *; unfold HC_refines in *; cleanup.
+
+    simpl in *; unfold TransactionToTransactionalDisk.Definitions.refines in *.
+    unfold Definitions.refines in *; simpl in *.
+    rewrite H13, H14.
+    unfold LogCache.cached_log_rep in *; cleanup.
+    repeat (split; eauto).
+  }
+  {
+    simpl; intros.
+
+
+    unfold refines_related in *; cleanup.
+    edestruct ATCD_AOE.
+    4: {
+      instantiate (1:= RFinished _ _).
+      instantiate (6:= []). 
+      unfold ATCD_reboot_list; simpl.
+      econstructor.
+      apply H.
+    }
+    all: try solve [simpl in *; eauto].
+    shelve.
+
+    edestruct ATCD_AOE.
+    4: {
+      instantiate (1:= RFinished _ _).
+      instantiate (6:= []). 
+      unfold ATCD_reboot_list; simpl.
+      econstructor.
+      apply H0.
+    }
+    all: try solve [simpl in *; eauto].
+    shelve.
+
+    edestruct ATCD_simulation.
+    2: apply H13.
+    all: eauto.
+    2:  unfold ATCD_reboot_list; simpl; econstructor; eauto.
+    shelve.
+
+    edestruct ATCD_simulation.
+    2: apply H14.
+    all: eauto.
+    2:  unfold ATCD_reboot_list; simpl; econstructor; eauto.
+    shelve.
+
+    simpl in *; cleanup; repeat invert_exec.
+
+    eapply_fresh lift2_invert_exec in H30;
+    eapply_fresh lift2_invert_exec in H31; cleanup.
+    
+    unfold refines_related in *; cleanup.
+    simpl in *; unfold HC_refines in *; cleanup.
+    simpl in *; unfold TransactionToTransactionalDisk.Definitions.refines in *.
+
+    eapply Transaction.read_finished in H26; eauto.
+    eapply Transaction.read_finished in H24; eauto.
+
+    unfold Inode.InodeAllocatorParams.bitmap_addr in *.
+    cleanup; repeat split_ors; cleanup; try lia.
+    erewrite InodeTS.inode_allocations_are_same with (s2:= fst (snd (snd x2))); eauto.
+    destruct_fresh (nth_error
+    (value_to_bits
+       (fst (snd (snd x2)) Inode.InodeAllocatorParams.bitmap_addr)) inum);
+    setoid_rewrite D; simpl.
+    2: {
+     eapply TS_eqv_impl.
+      apply ATCD_TS_ret.
+      shelve.
+    }
+    destruct b; simpl.
+    2: {
+     eapply TS_eqv_impl.
+      apply ATCD_TS_ret.
+      shelve.
+    }
+    eapply ATCD_TS_compositional; simpl.
+    2: intros; apply ATCD_TS_ret.
+    intros; eapply TS_eqv_impl.
+    eapply ATCD_TS_Transaction_read.
+    lia.
+    shelve.
+    intros; shelve.
+
+    destruct (block_allocator_empty inum); 
+    rewrite H18;
+    eapply TS_eqv_impl;
+    try apply ATCD_TS_ret.
+    shelve.
+    shelve.
+  }
+  {
+    simpl; intros; cleanup; eauto.
+    unfold refines_related in *; cleanup.
+    edestruct ATCD_AOE.
+    4: {
+      instantiate (1:= RFinished _ _).
+      instantiate (6:= []). 
+      unfold ATCD_reboot_list; simpl.
+      econstructor.
+      apply H.
+    }
+    all: try solve [simpl in *; eauto].
+    shelve.
+
+    edestruct ATCD_AOE.
+    4: {
+      instantiate (1:= RFinished _ _).
+      instantiate (6:= []). 
+      unfold ATCD_reboot_list; simpl.
+      econstructor.
+      apply H0.
+    }
+    all: try solve [simpl in *; eauto].
+    shelve.
+
+    edestruct ATCD_simulation.
+    2: apply H13.
+    all: eauto.
+    2:  unfold ATCD_reboot_list; simpl; econstructor; eauto.
+    shelve.
+
+    edestruct ATCD_simulation.
+    2: apply H14.
+    all: eauto.
+    2:  unfold ATCD_reboot_list; simpl; econstructor; eauto.
+    shelve.
+
+    simpl in *; cleanup; repeat invert_exec.
+
+    eapply_fresh lift2_invert_exec in H30;
+    eapply_fresh lift2_invert_exec in H31; cleanup.
+
+    simpl in *; unfold HC_refines in *; cleanup.
+    simpl in *; unfold TransactionToTransactionalDisk.Definitions.refines in *.
+
+    eapply Transaction.read_finished in H26; eauto.
+    eapply Transaction.read_finished in H24; eauto.
+
+    unfold Inode.InodeAllocatorParams.bitmap_addr in *.
+    pose proof Inode.InodeAllocatorParams.blocks_fit_in_disk.
+    cleanup; repeat split_ors; cleanup; try lia; eauto.
+    
+    shelve.
+  }
+}
+Unshelve.
+all: 
+try match goal with
+| [|- not_init _ ] =>
+  unfold Transaction.read;
+  destruct (Compare_dec.lt_dec Inode.InodeAllocatorParams.bitmap_addr
+  data_length); simpl; intuition eauto;
+  try destruct (Transaction.get_first t Inode.InodeAllocatorParams.bitmap_addr); 
+  simpl; intuition eauto; 
+  try match goal with
+  | [H: eq_dep _ _ _ _ _ _ |- _] =>
+  inversion H
+  end
+end.
+5: instantiate (5 := fun _ _ s0 s3 => 
+equivalent_for_recovery txns1 txns2 Log.Current_Part hdr1 hdr2 s0 s3 /\
+(Transaction.get_first (fst (snd s0)) (inode_blocks_start + S inum) = None <->
+ Transaction.get_first (fst (snd s3)) (inode_blocks_start + S inum) = None) /\
+(fst (snd (snd s0)) (data_start + (inode_blocks_start + S inum)) = None <->
+ fst (snd (snd s3)) (data_start + (inode_blocks_start + S inum)) = None) /\
+fst (snd (snd s0)) =
+Mem.list_upd_batch empty_mem (map Log.addr_list txns1)
+  (map Log.data_blocks txns1) /\
+fst (snd (snd s3)) =
+Mem.list_upd_batch empty_mem (map Log.addr_list txns2)
+  (map Log.data_blocks txns2)); simpl; intuition eauto.
+5: simpl; intuition eauto.
+9: simpl; intuition eauto.
+5: simpl; intuition eauto.
+14: simpl; intuition eauto.
+10: simpl; intuition eauto.
+5: {
+  (*
+  instantiate (1:= hdr2).
+  instantiate (1:= hdr1).
+  instantiate (1:= txns2).
+  instantiate (1:= txns1).
+  *)
+  simpl; intuition eauto.
+  simpl in *.
+
+  simpl; intros; cleanup; eauto.
+  unfold refines_related in *; cleanup.
+  edestruct ATCD_AOE.
+    4: {
+      instantiate (1:= RFinished _ _).
+      instantiate (6:= []). 
+      unfold ATCD_reboot_list; simpl.
+      econstructor.
+      apply H18.
+    }
+    all: try solve [simpl in *; eauto].
+    shelve.
+    simpl.
+    unfold HC_refines; simpl.
+    unfold HC_refines; simpl.
+    unfold Definitions.refines, LogCache.cached_log_rep.
+    unfold Log.log_rep, Log.log_header_rep, Log.log_rep_general.
+    unfold equivalent_for_recovery in *; cleanup.
+    eexists (_, (_, _)); simpl; intuition eauto.
+    eexists; simpl; intuition eauto.
+
+    edestruct ATCD_AOE.
+    4: {
+      instantiate (1:= RFinished _ _).
+      instantiate (6:= []). 
+      unfold ATCD_reboot_list; simpl.
+      econstructor.
+      apply H26.
+    }
+    all: try solve [simpl in *; eauto].
+    shelve.
+    simpl.
+    unfold HC_refines; simpl.
+    unfold HC_refines; simpl.
+    unfold Definitions.refines, LogCache.cached_log_rep.
+    unfold Log.log_rep, Log.log_header_rep, Log.log_rep_general.
+    unfold equivalent_for_recovery in *; cleanup.
+    eexists (_, (_, _)); simpl; intuition eauto.
+    eexists; simpl; intuition eauto.
+
+    unfold equivalent_for_recovery in *; cleanup.
+    edestruct ATCD_simulation.
+    2: apply H35.
+    all: eauto.
+    3:  unfold ATCD_reboot_list; simpl; econstructor; eauto.
+    shelve.
+    unfold Simulation.Definitions.refines; simpl.
+    unfold HC_refines; simpl.
+    unfold HC_refines; simpl.
+    unfold Definitions.refines, LogCache.cached_log_rep.
+    unfold Log.log_rep, Log.log_header_rep, Log.log_rep_general.
+    instantiate (1:= (_, (_, _))); simpl; intuition eauto.
+    eexists; simpl; intuition eauto.
+
+    edestruct ATCD_simulation.
+    2: apply H44.
+    all: eauto.
+    3:  unfold ATCD_reboot_list; simpl; econstructor; eauto.
+    shelve.
+    unfold Simulation.Definitions.refines; simpl.
+    unfold HC_refines; simpl.
+    unfold HC_refines; simpl.
+    unfold Definitions.refines, LogCache.cached_log_rep.
+    unfold Log.log_rep, Log.log_header_rep, Log.log_rep_general.
+    instantiate (1:= (_, (_, _))); simpl; intuition eauto.
+    eexists; simpl; intuition eauto.
+
+    simpl in *; cleanup_no_match; repeat invert_exec.
+
+    repeat invert_lift2.
+    simpl in *; unfold HC_refines in *; cleanup.
+    simpl in *; unfold TransactionToTransactionalDisk.Definitions.refines in *.
+
+    repeat cleanup_pairs.
+    (*
+    eapply Transaction.read_finished in H80; eauto.
+    eapply Transaction.read_finished in H81; eauto.
+
+    cleanup; repeat cleanup_pairs.
+    
+    repeat match goal with
+    |[H: _ \/ _|- _] =>
+    clear H
+    end.
+
+    unfold HC_refines in *; simpl in *; cleanup.
+    unfold Definitions.refines, LogCache.cached_log_rep in *.
+    unfold Log.log_rep, Log.log_header_rep, Log.log_rep_general in *.
+    cleanup.
+
+    eexists (_, (_, _)), (_, (_, _)); simpl; split.
+    intuition eauto.
+    do 2 eexists; split.
+    eauto.
+    *)
+    admit.
+}
+Admitted.
+
+
+Lemma ATCD_TS_DiskAllocator_read:
+    forall n a1 a2 u u' txns1 txns2 hdr1 hdr2,
+    (a1 < File.DiskAllocatorParams.num_of_blocks <-> a2 < File.DiskAllocatorParams.num_of_blocks) ->
+    (File.DiskAllocatorParams.bitmap_addr + S a1 <
+    data_length <->
+    File.DiskAllocatorParams.bitmap_addr + S a2 <
+    data_length) ->
+    Termination_Sensitive u
+  (Simulation.Definitions.compile
+     ATCD_Refinement
+     (Simulation.Definitions.compile
+    ATC_Refinement
+     (@lift_L2 AuthenticationOperation _ TD _
+     (File.DiskAllocator.read a1))))
+  (Simulation.Definitions.compile
+     ATCD_Refinement
+     (Simulation.Definitions.compile
+    ATC_Refinement
+     (@lift_L2 AuthenticationOperation _ TD _
+     (File.DiskAllocator.read a2))))
+  (Simulation.Definitions.compile
+     ATCD_Refinement
+     (Simulation.Definitions.compile
+    ATC_Refinement
+     (Simulation.Definitions.compile
+        FD.refinement
+        (| Recover |))))
+        (refines_valid ATCD_Refinement
+        (refines_valid ATC_Refinement
+       AD_valid_state))
+  (fun s1 s2 => equivalent_for_recovery txns1 txns2 Log.Current_Part hdr1 hdr2 s1 s2 /\
+  refines_related ATCD_Refinement (fun s1 s2 => refines_related ATC_Refinement
+  (fun s1 s2  => exists s1a s2a, 
+  File.files_inner_rep s1a (fst (snd (snd s1))) /\ 
+  File.files_inner_rep s2a (fst (snd (snd s2))) /\ 
+  FD_related_states u' None s1a s2a) s1 s2 /\
+  (forall a, 
+     Transaction.get_first (fst (snd s1)) a = None <-> 
+     Transaction.get_first (fst (snd s2)) a = None) /\
+  (Transaction.get_first (fst (snd s1)) (File.DiskAllocatorParams.bitmap_addr + S a1) = None <-> 
+   Transaction.get_first (fst (snd s2)) (File.DiskAllocatorParams.bitmap_addr + S a2) = None) /\
+   nth_error
+            (value_to_bits
+               (upd_batch (snd (snd s1)) (rev (map fst (fst (snd s1))))
+               (rev (map snd (fst (snd s1)))) File.DiskAllocatorParams.bitmap_addr)) a1 =
+               nth_error
+            (value_to_bits
+               (upd_batch (snd (snd s2)) (rev (map fst (fst (snd s2))))
+               (rev (map snd (fst (snd s2)))) File.DiskAllocatorParams.bitmap_addr)) a2) s1 s2)
+  (ATCD_reboot_list n).
+  Proof.
+    unfold File.DiskAllocator.read; intros.
+    destruct (Compare_dec.lt_dec a1 File.DiskAllocatorParams.num_of_blocks);
+    destruct (Compare_dec.lt_dec a2 File.DiskAllocatorParams.num_of_blocks);
+    try lia.
+    2: intros; eapply TS_eqv_impl; [apply ATCD_TS_ret | shelve].
+    simpl.
+    eapply ATCD_TS_compositional.
+
+    intros; eapply TS_eqv_impl.
+    eapply ATCD_TS_Transaction_read.
+    shelve.
+    shelve.
+    intros; cleanup; eauto.
+    2: shelve.
+    intros.
+
+    intros; unfold refines_related in *; cleanup.
+    intros; unfold refines_related in *; cleanup.
+      eapply_fresh ATCD_oracle_refines_finished in H1; eauto.
+      eapply_fresh ATCD_oracle_refines_finished in H2; eauto.
+      cleanup.
+
+      eapply_fresh ATCD_exec_lift_finished in H1; eauto;
+      try solve [apply TransactionToTransactionalDisk.Refinement.TC_to_TD_core_simulation_finished];
+      try solve [apply TransactionToTransactionalDisk.Refinement.TC_to_TD_core_simulation_crashed].
+      cleanup.
+      eapply_fresh ATCD_exec_lift_finished in H2; eauto;
+      try solve [apply TransactionToTransactionalDisk.Refinement.TC_to_TD_core_simulation_finished];
+      try solve [apply TransactionToTransactionalDisk.Refinement.TC_to_TD_core_simulation_crashed].
+      cleanup.
+      simpl in *.
+      eapply_fresh ATCD_oracle_refines_impl_eq in H14; eauto.
+      2: shelve. (* eapply have_same_structure_get_owner; eauto. *)
+      2: apply TC_oracle_refines_operation_eq.
+      cleanup.
+
+      clear H1 H2.
+    repeat invert_lift2; cleanup.
+    apply HC_map_ext_eq in H1; subst.
+    unfold HC_refines in *; simpl in *; cleanup.
+
+    unfold TransactionToTransactionalDisk.Definitions.refines in *.
+    eapply Transaction.read_finished in H18; eauto.
+    eapply Transaction.read_finished in H21; eauto.
+    cleanup; repeat split_ors; cleanup; try lia.
+    unfold Transaction.transaction_rep in *; cleanup.
+    setoid_rewrite H9.
+    destruct_fresh (nth_error
+    (value_to_bits
+       (upd_batch (snd (snd x0)) (rev (map fst (fst (snd x0))))
+          (rev (map snd (fst (snd x0))))
+          File.DiskAllocatorParams.bitmap_addr)) a2); setoid_rewrite D.
+          2: intros; eapply TS_eqv_impl; [apply ATCD_TS_ret | shelve].
+    {
+      destruct b.
+      2: intros; eapply TS_eqv_impl; [apply ATCD_TS_ret | shelve].
+      eapply ATCD_TS_compositional.
+      2: intros; eapply TS_eqv_impl; [apply ATCD_TS_ret | shelve].
+      intros; simpl; 
+      eapply TS_eqv_impl; [apply ATCD_TS_Transaction_read; eauto | shelve].
+      shelve.
+    }
+    {
+      edestruct (block_allocator_empty a1);
+      edestruct (block_allocator_empty a2);
+      cleanup;  (eapply TS_eqv_impl; [apply ATCD_TS_ret | shelve]).
+    }
+  Admitted.
