src/Noninterference/LoggedDisk/TS/ATCD_TS_BatchOperations.v
@@ -1,203 +1,277 @@
-Require Import Eqdep Lia Framework FSParameters CryptoDiskLayer BatchOperations.
+Require Import Eqdep Lia Framework FSParameters FileDiskLayer. (* LoggedDiskLayer TransactionCacheLayer TransactionalDiskLayer. *)
+Require Import FileDiskNoninterference FileDiskRefinement.
+Require Import ATCDLayer FileDisk.TransferProofs ATCD_Simulation ATCD_AOE.
+Require Import Not_Init HSS ATCD_ORS.
+Require Import ATCD_TS_Recovery ATCD_TS_Common ATCD_TS_Operations.
 
+Import FileDiskLayer.
 Set Nested Proofs Allowed.
+Opaque File.recover.
 
-  
-  Lemma BatchOperations_TS_hash_all:
-  forall u l1 l2 s1 s2 o s1' t h1 h2,
-  exec (CryptoDiskLang) u o s1 
-  (hash_all h1 l1)
-       (Finished s1' t) ->
+
+Lemma ATCD_TS_BatchOperations_encrypt_all:
+  forall n u k l1 l2 txns1 txns2 hdr1 hdr2,
   length l1 = length l2 ->
-  consistent_with_upds (snd (fst (fst s2))) (rolling_hash_list h2 l2) (combine (h2:: rolling_hash_list h2 l2) l2) ->
-  exists s2' t,
-  exec (CryptoDiskLang) u o s2 
-  (hash_all h2 l2)
-       (Finished s2' t).
-  Proof.
-    induction l1; destruct l2; simpl in *; try lia;
-    intros; repeat invert_exec_no_match.
-    do 2 eexists; repeat econstructor.
-    simpl in *.
-    edestruct IHl1.
-    eauto.
-    3:{
-      simpl in *; logic_clean.
-      do 2 eexists; repeat econstructor; eauto.
-      rewrite cons_app.
-      repeat (econstructor; eauto).
+Termination_Sensitive u
+(@lift_L2 AuthenticationOperation _ TCDLang _
+  (@lift_L2 _ _ CachedDiskLang _
+     (|CDDP| BatchOperations.encrypt_all k l1)))
+(@lift_L2 AuthenticationOperation _ TCDLang _
+     (@lift_L2 _ _ CachedDiskLang _
+        (|CDDP| BatchOperations.encrypt_all k l2)))
+   (Simulation.Definitions.compile
+     ATCD_Refinement
+     (Simulation.Definitions.compile
+   ATC_Refinement
+   (Simulation.Definitions.compile
+      FD.refinement
+      (| Recover |))))
+  (refines_valid ATCD_Refinement
+  (refines_valid ATC_Refinement AD_valid_state)) 
+  (fun s1 s2 => equivalent_for_recovery txns1 txns2
+  Log.Current_Part hdr1 hdr2 s1 s2 /\
+  (forall x, 
+  consistent_with_upds (snd (fst (snd (snd (snd s1))))) (firstn x (map (encrypt k) l1)) (firstn x (map (fun v => (k, v)) l1)) ->
+  consistent_with_upds (snd (fst (snd (snd (snd s2))))) (firstn x (map (encrypt k) l2)) (firstn x (map (fun v => (k, v)) l2))))
+(ATCD_reboot_list n).
+Proof.
+   unfold Termination_Sensitive, ATCD_reboot_list; 
+   intros; destruct n;
+   repeat invert_exec.
+   {
+      repeat invert_lift2; cleanup.
+      destruct s2, s0, s2, s3.
+
+      eapply_fresh BatchOperations.encrypt_all_finished in H8; cleanup; eauto.
+      eapply BatchOperations_TS_encrypt_all in H8; eauto; cleanup.
+      eexists (RFinished _ _).
+      repeat econstructor; eauto.
+      repeat eapply lift2_exec_step; eauto.
+      specialize (c (length l1)).
+      do 4 rewrite firstn_oob in c.
+      simpl in *.
+      eapply c; eauto.
+      all: repeat rewrite map_length; lia.
     }
-    eauto.
-    simpl; eauto.
-  Qed.
+    {
+      repeat invert_lift2; cleanup.
+      destruct s2, s0, s2, s3.
 
-  Lemma BatchOperations_TS_read_consecutive:
-  forall u n s1 s2 o s1' t h1 h2,
-  exec (CryptoDiskLang) u o s1 
-  (read_consecutive h1 n)
-       (Finished s1' t) ->
-       h2 + n < disk_size ->
-  exists s2' t,
-  exec (CryptoDiskLang) u o s2 
-  (read_consecutive h2 n)
-       (Finished s2' t).
-  Proof.
-    induction n; simpl in *; try lia;
-    intros; repeat invert_exec_no_match.
-    do 2 eexists; repeat econstructor.
-    simpl in *.
-    edestruct IHn.
-    eauto.
-    2:{
-      simpl in *; logic_clean.
-      do 2 eexists; repeat econstructor; eauto.
-      rewrite cons_app.
-      repeat (econstructor; eauto).
-      lia.
+      eapply_fresh BatchOperations.encrypt_all_crashed in H8; cleanup.
+      eapply BatchOperations_TS_encrypt_all_crashed in H8; eauto; cleanup.
+      eapply_fresh BatchOperations.encrypt_all_crashed in H8; cleanup.
+      repeat cleanup_pairs.
+      simpl in *.
+       edestruct ATCD_TS_recovery.
+       3: eauto.
+       3: shelve. (* eapply equivalent_for_recovery_after_reboot; eauto. *)
+ 
+       3: {
+          eexists (Recovered _); econstructor; eauto.
+      repeat eapply lift2_exec_step_crashed; eauto.
+      }
+
+      all: try solve [unfold AD_valid_state, 
+      refines_valid, FD_valid_state; 
+      intros; simpl; eauto].
     }
-    lia.
-  Qed.
+    Unshelve.
+    all: try exact ATCDLang.
+    6: {
+      unfold equivalent_for_recovery in *; simpl in *;
+      cleanup.
+      eexists (_, (_, _)), (_, (_,_)); split.
+      simpl; intuition eauto.
+      rewrite e2 in *;
+      do 2 eexists; intuition eauto.
+      eapply RepImplications.log_rep_explicit_after_reboot in l0; simpl in *.
+      eapply RepImplications.log_rep_explicit_consistent_with_upds; eauto.
+      eapply select_total_mem_synced in H3; eauto.
+      
+      simpl. split.
+      repeat split.
+      do 2 eexists; split.
+      eapply RepImplications.log_rep_explicit_after_reboot in l; simpl in *.
+      eapply RepImplications.log_rep_explicit_consistent_with_upds; eauto.
+      all: intuition eauto.
+      eapply select_total_mem_synced in H3; eauto.
+    }
+Qed.
 
-
-  Lemma BatchOperations_TS_decrypt_all:
-forall u l1 l2 k1 k2 s1 s2 o s1' t,
-
-exec (CryptoDiskLang) u o s1 
-(decrypt_all k1 l1)
-     (Finished s1' t) ->
-
-length l1 = length l2 ->
-
-consistent_with_upds (snd (fst s2)) l2 (map (fun ev => (k2, decrypt k2 ev)) l2) ->
-
-exists s2' t,
-exec (CryptoDiskLang) u o s2 (decrypt_all k2 l2) (Finished s2' t).
+Lemma ATCD_TS_BatchOperations_hash_all:
+  forall n u l1 l2 h1 h2 txns1 txns2 hdr1 hdr2,
+  length l1 = length l2 ->
+Termination_Sensitive u
+(@lift_L2 AuthenticationOperation _ TCDLang _
+  (@lift_L2 _ _ CachedDiskLang _
+     (|CDDP| BatchOperations.hash_all h1 l1)))
+(@lift_L2 AuthenticationOperation _ TCDLang _
+     (@lift_L2 _ _ CachedDiskLang _
+        (|CDDP| BatchOperations.hash_all h2 l2)))
+   (Simulation.Definitions.compile
+     ATCD_Refinement
+     (Simulation.Definitions.compile
+   ATC_Refinement
+   (Simulation.Definitions.compile
+      FD.refinement
+      (| Recover |))))
+  (refines_valid ATCD_Refinement
+  (refines_valid ATC_Refinement AD_valid_state)) 
+  (fun s1 s2 => equivalent_for_recovery txns1 txns2
+  Log.Current_Part hdr1 hdr2 s1 s2 /\
+  (forall x,
+  consistent_with_upds (snd (fst (fst (snd (snd (snd s1)))))) 
+  (firstn x (rolling_hash_list h1 l1))
+  (firstn x (combine (h1 :: rolling_hash_list h1 l1) l1)) ->
+  consistent_with_upds (snd (fst (fst (snd (snd (snd s2)))))) 
+  (firstn x (rolling_hash_list h2 l2))
+  (firstn x (combine (h2 :: rolling_hash_list h2 l2) l2))))
+(ATCD_reboot_list n).
 Proof.
-     induction l1; 
-     destruct l2; simpl; intros; 
-     try lia;repeat invert_exec.
-     repeat econstructor.
-     eapply IHl1 in H; cleanup.
-     do 2 eexists; econstructor; eauto.
-     do 3 econstructor; eauto.
-     repeat econstructor; eauto.
-     all: simpl; eauto.
+   unfold Termination_Sensitive, ATCD_reboot_list; 
+   intros; destruct n;
+   repeat invert_exec.
+   {
+      repeat invert_lift2; cleanup.
+      destruct s2, s0, s2, s3.
+      eapply BatchOperations_TS_hash_all in H8; eauto; cleanup.
+      eexists (RFinished _ _).
+      repeat econstructor; eauto.
+      repeat eapply lift2_exec_step; eauto.
+      eapply BatchOperations.hash_all_finished in H8; cleanup; eauto.
+      specialize (c (length l1)).
+      do 4 rewrite firstn_oob in c.
+      apply c; eauto.
+      all: repeat rewrite combine_length; try lia.
+
+      
+
+      all: rewrite rolling_hash_list_length; lia.
+    }
+    {
+      repeat invert_lift2; cleanup.
+      destruct s2, s0, s2, s3.
+      eapply_fresh BatchOperations_TS_hash_all_crashed in H8; eauto; cleanup.
+      eapply BatchOperations.hash_all_crashed in H8; cleanup.
+      eapply_fresh BatchOperations.hash_all_crashed in H2; cleanup.
+      repeat cleanup_pairs.
+      simpl in *.
+       edestruct ATCD_TS_recovery.
+       3: eauto.
+       3: shelve. (* eapply equivalent_for_recovery_after_reboot; eauto. *)
+       3: {
+         eexists (Recovered _); econstructor; eauto.
+         repeat eapply lift2_exec_step_crashed; eauto.
+       }
+       (* 3: repeat cleanup_pairs; eauto. *)
+       all: try solve [unfold AD_valid_state, 
+       refines_valid, FD_valid_state; 
+       intros; simpl; eauto].
+    }
+    Unshelve.
+    all: try exact ATCDLang.
+    6: {
+      unfold equivalent_for_recovery in *; simpl in *;
+      cleanup_no_match.
+      eexists (_, (_, _)), (_, (_,_)); split.
+      simpl; intuition eauto.
+      rewrite e2 in *;
+      do 2 eexists; intuition eauto.
+      eapply RepImplications.log_rep_explicit_after_reboot in l4; simpl in *.
+      eapply RepImplications.log_rep_explicit_consistent_with_upds_hashmap; eauto.
+      eapply select_total_mem_synced in H4; eauto.
+      
+      simpl. split.
+      repeat split.
+      do 2 eexists; split.
+      eapply RepImplications.log_rep_explicit_after_reboot in l3; simpl in *.
+      eapply RepImplications.log_rep_explicit_consistent_with_upds_hashmap; eauto.
+      all: intuition eauto.
+      eapply select_total_mem_synced in H4; eauto.
+    }
 Qed.
 
 
-(*************************** Crashed TS ********************)
-
-Lemma BatchOperations_TS_hash_all_crashed:
-forall u l1 l2 s1 s2 o s1' h1 h2,
-exec (CryptoDiskLang) u o s1 
-(hash_all h1 l1) (Crashed s1') ->
-length l1 = length l2 ->
-consistent_with_upds (snd (fst (fst s2))) (rolling_hash_list h2 l2) (combine (h2:: rolling_hash_list h2 l2) l2) ->
-exists s2',
-exec (CryptoDiskLang) u o s2 
-(hash_all h2 l2) (Crashed s2').
+Lemma ATCD_TS_BatchOperations_write_batch:
+  forall n u la1 la2 lv1 lv2 txns1 txns2 hdr1 hdr2,
+  length la1 = length la2 ->
+  length lv1 = length lv2 ->
+  length la2 = length lv2 ->
+  Forall (fun a => a < disk_size) la2 ->
+Termination_Sensitive u
+(@lift_L2 AuthenticationOperation _ TCDLang _
+  (@lift_L2 _ _ CachedDiskLang _
+     (|CDDP| BatchOperations.write_batch la1 lv1)))
+(@lift_L2 AuthenticationOperation _ TCDLang _
+     (@lift_L2 _ _ CachedDiskLang _
+        (|CDDP| BatchOperations.write_batch la2 lv2)))
+   (Simulation.Definitions.compile
+     ATCD_Refinement
+     (Simulation.Definitions.compile
+   ATC_Refinement
+   (Simulation.Definitions.compile
+      FD.refinement
+      (| Recover |))))
+  (refines_valid ATCD_Refinement
+  (refines_valid ATC_Refinement AD_valid_state)) 
+  (equivalent_for_recovery txns1 txns2
+  Log.Current_Part hdr1 hdr2)
+(ATCD_reboot_list n).
 Proof.
-  induction l1; destruct l2; simpl in *; try lia;
-  intros; repeat invert_exec_no_match.
-  eexists; repeat econstructor.
+   unfold Termination_Sensitive, ATCD_reboot_list; 
+   intros; destruct n;
+   repeat invert_exec.
+   {
+      repeat invert_lift2; cleanup.
+      destruct s2, s0, s2, s3.
+      eapply BatchOperations_TS_write_batch in H12; cleanup.
+      eexists (RFinished _ _).
+      repeat econstructor; eauto.
+      repeat eapply lift2_exec_step; eauto.
+      all: eauto.
+    }
+    {
+      repeat invert_lift2; cleanup.
+      destruct s2, s0, s2, s3.
+      eapply_fresh BatchOperations_TS_write_batch_crashed in H12; cleanup.
+      eapply BatchOperations.write_batch_crashed in H12; cleanup.
+      eapply_fresh BatchOperations.write_batch_crashed in H5; cleanup.
+      simpl in *.
+       edestruct ATCD_TS_recovery.
+       3: eauto.
+       3: shelve. (* eapply equivalent_for_recovery_after_reboot; eauto. *)
+      3: { 
+         eexists (Recovered _); econstructor; eauto.
+      repeat eapply lift2_exec_step_crashed; eauto.
+    }
+    all: try solve [unfold AD_valid_state, 
+      refines_valid, FD_valid_state; 
+      intros; simpl; eauto].
 
-  simpl in *; split_ors; cleanup_no_match.
-  repeat invert_exec.
-  eexists; repeat econstructor.
-  repeat invert_exec_no_match.
-  simpl in *; split_ors; cleanup_no_match.
-  edestruct IHl1.
-  eauto.
-  3:{
-    eexists; rewrite cons_app.
-    repeat (econstructor; eauto).
-  }
-  eauto.
-  simpl; eauto.
+    Unshelve.
+    all: try exact ATCDLang.
+    6: {
+       (* probably need to add the fact that 
+       it is written to the end of the log *)
+      admit. (*
+      unfold equivalent_for_recovery in *; simpl in *;
+      cleanup_no_match.
+      eexists (_, (_, _)), (_, (_,_)); split.
+      simpl; intuition eauto.
+      do 2 eexists; intuition eauto.
 
-  repeat invert_exec_no_match.
-  eapply BatchOperations_TS_hash_all in H3; cleanup_no_match.
-  eexists; rewrite cons_app.
-repeat (econstructor; eauto).
-eauto.
-simpl; eauto.
-Qed.
-
-Lemma BatchOperations_TS_read_consecutive_crashed:
-forall u n s1 s2 o s1' h1 h2,
-exec (CryptoDiskLang) u o s1 
-(read_consecutive h1 n)
-     (Crashed s1') ->
-     h2 + n < disk_size ->
-exists s2',
-exec (CryptoDiskLang) u o s2 
-(read_consecutive h2 n) (Crashed s2').
-Proof.
-  induction n; simpl in *; try lia;
-  intros; repeat invert_exec_no_match.
-  eexists; repeat econstructor.
-
-  simpl in *; split_ors; cleanup_no_match.
-  repeat invert_exec.
-  eexists; repeat econstructor.
-  repeat invert_exec_no_match.
-  simpl in *; split_ors; cleanup_no_match.
-
-  edestruct IHn.
-  eauto.
-  2:{
-    eexists; rewrite cons_app.
-    repeat (econstructor; eauto).
-    lia.
-  }
-  lia.
-
-
-  repeat invert_exec_no_match.
-  eapply BatchOperations_TS_read_consecutive in H1; cleanup_no_match.
-  eexists; rewrite cons_app.
-repeat (econstructor; eauto).
-all: lia.
-Qed.
-
-
-Lemma BatchOperations_TS_decrypt_all_crashed:
-forall u l1 l2 k1 k2 s1 s2 o s1',
-
-exec (CryptoDiskLang) u o s1 
-(decrypt_all k1 l1)
-   (Crashed s1') ->
-
-length l1 = length l2 ->
-
-consistent_with_upds (snd (fst s2)) l2 (map (fun ev => (k2, decrypt k2 ev)) l2) ->
-
-exists s2',
-exec (CryptoDiskLang) u o s2 (decrypt_all k2 l2) (Crashed s2').
-Proof.
-   induction l1; 
-   destruct l2; simpl; intros; 
-   try lia;repeat invert_exec.
-   repeat econstructor.
-
-   simpl in *; split_ors; cleanup_no_match.
-  repeat invert_exec.
-  eexists; repeat econstructor.
-  repeat invert_exec_no_match.
-  simpl in *; split_ors; cleanup_no_match.
-  edestruct IHl1.
-  eauto.
-  3:{
-    eexists; rewrite cons_app.
-    repeat (econstructor; eauto).
-  }
-  eauto.
-  simpl; eauto.
-
-  repeat invert_exec_no_match.
-  eapply BatchOperations_TS_decrypt_all in H3; cleanup_no_match.
-  eexists; rewrite cons_app.
-repeat (econstructor; eauto).
-eauto.
-simpl; eauto.
-Qed.
+      Search Log.log_rep_explicit upd_batch_set.
+      eapply RepImplications.log_rep_explicit_after_reboot in l4; simpl in *.
+      eapply RepImplications.log_rep_explicit_consistent_with_upds_hashmap; eauto.
+      eapply select_total_mem_synced in H3; eauto.
+      
+      simpl. split.
+      repeat split.
+      do 2 eexists; split.
+      eapply RepImplications.log_rep_explicit_after_reboot in l3; simpl in *.
+      eapply RepImplications.log_rep_explicit_consistent_with_upds_hashmap; eauto.
+      all: intuition eauto.
+      eapply select_total_mem_synced in H3; eauto.
+      *)
+    }
+Admitted.
