src/Noninterference/LoggedDisk/TS/ATCD_TS_Common.v
@@ -2,445 +2,39 @@ Require Import Eqdep Lia Framework FSParameters FileDiskLayer. (* LoggedDiskLaye
 Require Import FileDiskNoninterference FileDiskRefinement.
 Require Import ATCLayer Not_Init HSS ATC_ORS ATC_Simulation ATC_AOE.
 Require Import ATCDLayer FileDisk.TransferProofs ATCD_Simulation ATCD_AOE ATCD_ORS.
-Require Import ATCD_TS_BatchOperations ATCD_TS_Log ATCD_TS_LogCache.
+Require Import ATCD_TS_Recovery.
 Import FileDiskLayer.
 Set Nested Proofs Allowed.
 
-
-(* TODO: Move to framework *)
-Lemma TS_explicit_and_inject:
-forall u s1 s2 T (p1 p2: ATCDLang.(prog) T) rec V 
-(R1 R2: state ATCDLang -> state ATCDLang -> Prop) l_grs,
-R2 s1 s2 ->
-Termination_Sensitive_explicit u s1 s2
-p1 p2 rec V (fun s1 s2 => R1 s1 s2 /\ R2 s1 s2) l_grs ->
-Termination_Sensitive_explicit u s1 s2
-p1 p2 rec V R1 l_grs.
-Proof.
-  unfold Termination_Sensitive_explicit; intros.
-  eapply H0; eauto.
-Qed.
-
-Lemma TS_explicit_to_TS:
-forall u T (p1 p2: ATCDLang.(prog) T) rec V 
-(R: state ATCDLang -> state ATCDLang -> Prop) l_grs,
-  (forall s1 s2, Termination_Sensitive_explicit u s1 s2
-p1 p2 rec V R l_grs) <->
-Termination_Sensitive u
-p1 p2 rec V R l_grs.
-Proof.
-  unfold Termination_Sensitive_explicit, Termination_Sensitive; intros.
-  intuition; eauto.
-Qed.
-
-Lemma TS_eqv_impl:
-forall u T (p1 p2: ATCDLang.(prog) T) rec V 
-(R1 R2: state ATCDLang -> state ATCDLang -> Prop) l_grs,
-Termination_Sensitive u p1 p2 rec V R1 l_grs ->
-(forall s1 s2, R2 s1 s2 -> R1 s1 s2) ->
-Termination_Sensitive u
-p1 p2 rec V R2 l_grs.
-Proof.
-  unfold Termination_Sensitive; intros.
-  intuition; eauto.
-Qed.
-
-
-
-
-Opaque LogCache.recover LogCache.init.
-Lemma test_core:
-forall u T (p: ATCCore.(operation) T) grs o o0 x s sa sa' r,
-@HC_token_refines _ _ _ TCDLang ATCDLang TCD_CoreRefinement T u s o grs o0 x ->
-Core.exec ATCCore u x sa o (Finished sa' r) ->
-ATCD_CoreRefinement.(Simulation.Definitions.refines_core) s sa ->
-exists s' r,
-exec ATCDLang u o0 s (ATCD_CoreRefinement.(Simulation.Definitions.compile_core) o) (Finished s' r).
-Proof.
-  intros; destruct o; simpl in *; cleanup.
-  {
-    invert_exec.
-    unfold HC_refines in *; cleanup.
-    eexists; repeat econstructor; eauto.
-    rewrite H; eauto.
-  }
-  {
-    invert_exec.
-    unfold HC_refines in *; cleanup.
-    destruct o;  simpl in *; cleanup.
-    {
-      specialize (H3 tt); cleanup.
-      unfold HC_refines in *; simpl in *; cleanup.
-      repeat invert_exec;
-      eexists; repeat econstructor; eauto.
-      (* rewrite <- H0; econstructor; eauto. *)
-    }
-    {
-      specialize (H3 tt); cleanup.
-      unfold HC_refines in *; simpl in *; cleanup.
-      specialize (H3 []); cleanup.
-      repeat invert_exec; simpl in *.
-      {
-        split_ors; cleanup; try congruence;
-      unfold HC_transform_oracle in *;
-      repeat cleanup_pairs;
-      do 2 eexists; 
-      repeat eapply lift2_exec_step; eauto.
-      }
-      {
-        split_ors; cleanup; try congruence;
-      unfold HC_transform_oracle in *;
-      repeat cleanup_pairs;
-      do 2 eexists; 
-      repeat eapply lift2_exec_step; eauto.
-      }
-      {
-        repeat (repeat split_ors; cleanup; try congruence);
-      unfold HC_transform_oracle in *;
-      repeat cleanup_pairs;
-      do 2 eexists; 
-      repeat eapply lift2_exec_step; eauto.
-
-      unfold Definitions.refines in *; cleanup.
-      apply H3 in H1; cleanup; 
-      split_ors; cleanup; try congruence.
-    }
-    {
-      clear H8.
-      repeat (repeat split_ors; cleanup; try congruence);
-      unfold HC_transform_oracle in *;
-      repeat cleanup_pairs;
-      do 2 eexists; 
-      repeat eapply lift2_exec_step; eauto.
-
-      unfold Definitions.refines in *; cleanup.
-      apply H3 in H1; cleanup; 
-      split_ors; cleanup; try congruence.
-    }
-    {
-        repeat (repeat split_ors; cleanup; try congruence);
-      unfold HC_transform_oracle in *;
-      repeat cleanup_pairs;
-      do 2 eexists; 
-      repeat eapply lift2_exec_step; eauto.
-    }
-    {
-        repeat (repeat split_ors; cleanup; try congruence);
-      unfold HC_transform_oracle in *;
-      repeat cleanup_pairs;
-      do 2 eexists; 
-      repeat eapply lift2_exec_step; eauto.
-    }
-  }
-}
-Unshelve.
-all: eauto.
-Qed.
-
-
-Lemma test:
-forall u T (p: ATCLang.(prog) T) grs o oa s sa sa' r,
-oracle_refines ATCDCore ATCCore ATCDLang ATCLang
-   ATCD_CoreRefinement T u s p (ATCD_reboot_f grs) o oa ->
-Language.exec' u oa sa p (Finished sa' r) ->
-ATCD_Refinement.(Simulation.Definitions.refines) s sa ->
-not_init p ->
-exists s' r,
-exec ATCDLang u o s (ATCD_Refinement.(Simulation.Definitions.compile) p) (Finished s' r).
-Proof.
-  induction p; simpl; intros.
-  {
-    clear H2.
-    simpl in *; cleanup.
-    invert_exec'' H0.
-    eapply test_core in H2; eauto.
-  }
-  {
-    invert_exec'' H0.
-    split_ors; repeat invert_exec; cleanup; try congruence;
-    eauto.
-  }
-  {
-    invert_exec'' H1.
-    split_ors; repeat invert_exec; cleanup; try congruence;
-    eauto.
-
-    eapply ATCD_exec_lift_crashed in H0; eauto.
-    cleanup.
-    exfalso; eapply finished_not_crashed_oracle_prefix.
-    eauto.
-    2: eauto.
-    rewrite app_assoc; eauto.
-
-
-    eapply_fresh ATCD_exec_lift_finished in H5; eauto.
-    cleanup.
-    eapply exec_finished_deterministic_prefix in H10; eauto; cleanup.
-    destruct x5.
-    eapply_fresh ATCD_exec_lift_finished in H6; eauto.
-    cleanup.
-    unify_execs; cleanup.
-    do 2 eexists; repeat econstructor; eauto.
-
-    eapply_fresh ATCD_exec_lift_crashed in H6; eauto.
-    cleanup.
-    unify_execs; cleanup.
-  }
-Unshelve.
-eauto.
-Qed.
-
-(*
-Lemma test3:
-forall u T (p: ATCLang.(prog) T) grs o oa s1 s2 s1' sa1 sa2 sa1' sa2' r r1 r2,
-oracle_refines ATCDCore ATCCore ATCDLang ATCLang
-   ATCD_CoreRefinement T u s1 p grs o oa ->
-Language.exec' u oa sa1 p (Finished sa1' r1) ->
-Language.exec' u oa sa2 p (Finished sa2' r2) ->
-exec ATCDLang u o s1 (ATCD_Refinement.(Simulation.Definitions.compile) p) (Finished s1' r) ->
-ATCD_Refinement.(Simulation.Definitions.refines) s1 sa1 ->
-ATCD_Refinement.(Simulation.Definitions.refines) s2 sa2 ->
-not_init p ->
-oracle_refines ATCDCore ATCCore ATCDLang ATCLang
-   ATCD_CoreRefinement T u s2 p grs o oa.
-Proof.
-  induction p; simpl; intros.
-  {
-    clear H5.
-    simpl in *; cleanup.
-    invert_exec'' H0.
-    invert_exec'' H1.
-    destruct o.
-    {
-      simpl in *; cleanup; eauto.
-    }
-    {
-      simpl in *; cleanup; eauto.
-      specialize (H1 tt).
-      destruct o.
-      {
-        simpl in *; cleanup; eauto.
-        eexists; intuition eauto.
-        do 2 eexists; intuition eauto.
-      }
-      {
-        simpl in *; cleanup; eauto.
-        specialize (H1 []).
-        simpl in *; cleanup.
-        eexists; intuition eauto.
-        do 2 eexists; intuition eauto.
-        do 2 eexists; intuition eauto.
-        destruct o; simpl in *.
-        {
-          repeat invert_exec;
-          repeat apply HC_map_ext_eq in H; subst.
-          split_ors; cleanup; try congruence.
-          left; do 2 eexists; intuition eauto.
-          unfold LogCache.read in *; 
-          cleanup; try lia; repeat invert_exec.
-          repeat econstructor; eauto.
-        }
-      }
-    }
-
-    eapply test_core in H2; eauto.
-  }
-  {
-    invert_exec'' H0.
-    split_ors; repeat invert_exec; cleanup; try congruence;
-    eauto.
-  }
-  {
-    invert_exec'' H1.
-    split_ors; repeat invert_exec; cleanup; try congruence;
-    eauto.
-
-    eapply ATCD_exec_lift_crashed in H0; eauto.
-    cleanup.
-    exfalso; eapply finished_not_crashed_oracle_prefix.
-    eauto.
-    2: eauto.
-    rewrite app_assoc; eauto.
-*)
-
-Lemma ATCD_TS_recovery:
-forall n u txns1 txns2 valid_part hdr1 hdr2,
-Termination_Sensitive u
-(Simulation.Definitions.compile
- ATCD_Refinement
-(Simulation.Definitions.compile
- ATC_Refinement
- File.recover))
-(Simulation.Definitions.compile
- ATCD_Refinement
-(Simulation.Definitions.compile
- ATC_Refinement
- File.recover))
- (Simulation.Definitions.compile
- ATCD_Refinement
- (Simulation.Definitions.compile
- ATC_Refinement
- File.recover))
-(refines_valid ATCD_Refinement
-  (refines_valid ATC_Refinement
- AD_valid_state))
-(fun s1 s2 => 
-exists sa1 sa2,
-(fst s1 = fst sa1 /\
- fst (snd s1) = fst (snd sa1) /\
- ((exists (hdr_blockset : set value) (log_blocksets : list (set value)),
- Log.log_rep_explicit Log.Hdr_Synced Log.Synced valid_part hdr1
-   txns1 hdr_blockset log_blocksets (snd (snd (snd s1))) /\
- (valid_part = Log.Old_Part ->
-  Log.hash (Log.current_part hdr1) <>
-  rolling_hash hash0
-    (firstn (Log.count (Log.current_part hdr1))
-       (map fst log_blocksets)))) /\
-    snd (snd sa1) =
-    total_mem_map fst
-      (shift (Nat.add data_start)
-         (list_upd_batch_set (snd (snd (snd (snd s1))))
-            (map Log.addr_list txns1) (map Log.data_blocks txns1))) /\
-    (forall a : nat,
-     a >= data_start -> snd (snd (snd (snd (snd s1))) a) = [])) /\
- (forall (a : addr) (vs : value * list value),
-  snd (snd (snd (snd s1))) a = vs -> snd vs = [])) /\
-(fst s2 = fst sa2 /\
- fst (snd s2) = fst (snd sa2) /\
- ((exists (hdr_blockset : set value) (log_blocksets : list (set value)),
- Log.log_rep_explicit Log.Hdr_Synced Log.Synced valid_part hdr2
-   txns2 hdr_blockset log_blocksets (snd (snd (snd s2))) /\
- (valid_part = Log.Old_Part ->
-  Log.hash (Log.current_part hdr2) <>
-  rolling_hash hash0
-    (firstn (Log.count (Log.current_part hdr2))
-       (map fst log_blocksets)))) /\
-    snd (snd sa2) =
-    total_mem_map fst
-      (shift (Nat.add data_start)
-         (list_upd_batch_set (snd (snd (snd (snd s2))))
-            (map Log.addr_list txns2) (map Log.data_blocks txns2))) /\
-    (forall a : nat,
-     a >= data_start -> snd (snd (snd (snd (snd s2))) a) = [])) /\
- (forall (a : addr) (vs : value * list value),
-  snd (snd (snd (snd s2))) a = vs -> snd vs = [])) /\ 
-length txns1 = length txns2 /\
-(valid_part = Log.Old_Part ->
-Log.count (Log.current_part hdr1) = Log.count (Log.current_part hdr2)) /\
-Forall2
-  (fun rec1 rec2 : Log.txn_record =>
-   Log.start rec1 = Log.start rec2 /\
-   Log.addr_count rec1 = Log.addr_count rec2 /\
-   Log.data_count rec1 = Log.data_count rec2) (map Log.record txns1)
-  (map Log.record txns2))
-(ATCD_reboot_list n).
-Proof.
-unfold Termination_Sensitive, ATCD_reboot_list; induction n.
-{
-  simpl; intros.
-  repeat invert_exec.
-  unfold AD_related_states, refines_valid in *.
-  cleanup.
-  Transparent File.recover.
-  unfold File.recover in *; simpl in *.
-  invert_exec'' H9; repeat invert_exec.
-  invert_exec'' H25; repeat invert_exec.
-  eapply lift2_invert_exec in H28; cleanup.
-  eapply lift2_invert_exec in H20; cleanup.
-  simpl in *.
-
-eapply LogCache_TS_recover in H21; cleanup.
-eexists (RFinished _ _); repeat econstructor.
-rewrite cons_app; repeat econstructor; eauto.
-apply lift2_exec_step; eauto.
-shelve.
-apply lift2_exec_step; eauto.
-intuition eauto.
-intuition eauto.
-all: eauto.
-}
-{
-  Opaque LogCache.recover.
-  intros.
-  repeat invert_exec.
-  simpl in *; cleanup; try tauto.
-  invert_exec'' H12; repeat invert_exec.
-  { (* Recover crashed*)
-    invert_exec'' H26; repeat invert_exec.
-    simpl in *.
-    eapply lift2_invert_exec_crashed in H29; cleanup.
-    eapply lift2_invert_exec_crashed in H21; cleanup.
-    simpl in *.
-    eapply_fresh LogCache_TS_recover_crashed in H22; try logic_clean.
-    edestruct IHn. 
-    3: eauto.
-
-    unfold AD_valid_state, 
-    refines_valid, FD_valid_state; 
-    intros; simpl; eauto.
-
-    unfold AD_valid_state, 
-    refines_valid, FD_valid_state; 
-    intros; simpl; eauto.
-  2: {
-    eexists (Recovered _); econstructor.
-    simpl in *.
-    rewrite cons_app.
-    econstructor.
-    repeat econstructor.
-    repeat apply lift2_exec_step_crashed; eauto.
-    shelve.
-    simpl; eauto.
-  }
-  simpl; shelve.
-  simpl in *; intuition eauto.
-  simpl in *; intuition eauto.
-  all: eauto.
-}
-{ (*Delete crashed*)
-  invert_exec'' H25; repeat invert_exec.
-  simpl in *.
-    edestruct IHn. 
-    3: eauto.
-
-    unfold AD_valid_state, 
-    refines_valid, FD_valid_state; 
-    intros; simpl; eauto.
-
-    unfold AD_valid_state, 
-    refines_valid, FD_valid_state; 
-    intros; simpl; eauto.
-
-  2: {
-    eexists (Recovered _); econstructor.
-    simpl in *.
-    repeat econstructor.
-    simpl; eauto.
-  }
-  simpl; shelve.
-}
-}
-Unshelve.
-all: try solve [exact (fun _ _ => True)].
-all: simpl; eauto.
-all: try solve [exact ATCDLang].
-all: admit. (* These are Log Cache crashed then reboot implies other stuff things *)
-Admitted.
+Ltac invert_lift2:=
+match goal with
+|[H: exec _ _ _ _ (lift_L2 _ _) (Finished _ _) |- _] =>
+eapply lift2_invert_exec in H; try logic_clean
+|[H: exec _ _ _ _ (lift_L2 _ _) (Crashed _) |- _] =>
+eapply lift2_invert_exec_crashed in H; try logic_clean
+|[H: Language.exec' _ _ _ (lift_L2 _ _) (Finished _ _) |- _] =>
+eapply lift2_invert_exec in H; try logic_clean
+|[H: Language.exec' _ _ _ (lift_L2 _ _) (Crashed _) |- _] =>
+eapply lift2_invert_exec_crashed in H; try logic_clean
+end.
 
 
 Lemma ATCD_TS_compositional:
 forall T (p1 p2: ATCDLang.(prog) T) 
 T' (p3 p4: T -> ATCDLang.(prog) T') 
-u n (R R': state ATCDLang -> state ATCDLang -> Prop),
+u n (R : state ATCDLang -> state ATCDLang -> Prop)
+(R': T -> T -> state ATCDLang -> state ATCDLang -> Prop),
 (forall n,
 Termination_Sensitive u p1 p2
 (Simulation.Definitions.compile
  ATCD_Refinement
  (Simulation.Definitions.compile
-    FD.refinement
-    (| Recover |)))
-(refines_valid ATCD_Refinement
- AD_valid_state) R
+ ATC_Refinement
+ File.recover))
+ (refines_valid ATCD_Refinement
+ (refines_valid ATC_Refinement
+AD_valid_state)) 
+R
 (ATCD_reboot_list n)) ->
 
 (forall n s1 s2 o s1' r1 s2' r2 ,
@@ -451,26 +45,28 @@ Termination_Sensitive u (p3 r1) (p4 r2)
 (Simulation.Definitions.compile
 ATCD_Refinement
 (Simulation.Definitions.compile
-  FD.refinement
-  (| Recover |)))
-(refines_valid ATCD_Refinement
-AD_valid_state)
-R'
+ ATC_Refinement
+ File.recover))
+  (refines_valid ATCD_Refinement
+  (refines_valid ATC_Refinement
+ AD_valid_state))
+(R' r1 r2)
 (ATCD_reboot_list n)) ->
 
 (forall s1 s2 o s1' r1 s2' r2 ,
 exec ATCDLang u o s1 p1 (Finished s1' r1) ->
 exec ATCDLang u o s2 p2 (Finished s2' r2) ->
 R s1 s2 ->
-R' s1' s2') ->
+R' r1 r2 s1' s2') ->
 Termination_Sensitive u (Bind p1 p3) (Bind p2 p4)
 (Simulation.Definitions.compile
 ATCD_Refinement
 (Simulation.Definitions.compile
-  FD.refinement
-  (| Recover |)))
-(refines_valid ATCD_Refinement
-AD_valid_state)
+ ATC_Refinement
+ File.recover))
+ (refines_valid ATCD_Refinement
+ (refines_valid ATC_Refinement
+AD_valid_state))
 R
 (ATCD_reboot_list n).
 Proof.
@@ -483,7 +79,7 @@ edestruct H.
 4: eauto.
 all: eauto.
 instantiate (1 := RFinished _ _).
-instantiate (3 := 0).
+instantiate (3 := []).
 simpl.
 econstructor; eauto.
 eauto.
@@ -497,7 +93,7 @@ all: unfold refines_valid, AD_valid_state; simpl;
      unfold refines_valid, FD_valid_state; simpl; eauto.
 
 instantiate (1 := RFinished _ _).
-instantiate (3 := 0).
+instantiate (3 := []).
 simpl.
 econstructor; eauto.
 simpl in *; invert_exec.
@@ -519,7 +115,7 @@ invert_exec'' H15.
   4: eauto.
   all: eauto.
   instantiate (1 := RFinished _ _).
-  instantiate (3 := 0).
+  instantiate (3 := []).
   simpl.
   econstructor; eauto.
   simpl in *; invert_exec.
@@ -531,7 +127,7 @@ all: unfold refines_valid, AD_valid_state; simpl;
      unfold refines_valid, FD_valid_state; simpl; eauto.
 
 instantiate (1 := Recovered _).
-instantiate (2 := S n).
+instantiate (2 := t::n).
 simpl.
 econstructor; eauto.
 simpl in *; invert_exec.
@@ -543,7 +139,7 @@ eexists (Recovered _); repeat econstructor; eauto.
   4: eauto.
   all: eauto.
   instantiate (1 := Recovered _).
-  instantiate (2 := S n).
+  instantiate (2 := t::n).
   simpl.
   econstructor; eauto.
   simpl in *; invert_exec.
@@ -553,55 +149,67 @@ eexists (Recovered _); repeat econstructor; eauto.
 Unshelve.
 all: try solve [exact (fun _ _ => True)].
 all: simpl; eauto.
-Qed.
+all: try solve [exact []].
+all: try solve [exact Log.header0].
+all: try solve [exact Log.Current_Part].
+all: admit. (* These are Log Cache crashed then reboot implies other stuff things *)
+Admitted.
 
 
 Lemma ATCD_TS_explicit_compositional:
 forall T (p1 p2: ATCDLang.(prog) T) 
 T' (p3 p4: T -> ATCDLang.(prog) T') 
-u n (R R': state ATCDLang -> state ATCDLang -> Prop) s1 s2,
-(forall n,
-Termination_Sensitive_explicit u s1 s2 p1 p2
+u n (R : state ATCDLang -> state ATCDLang -> Prop)
+(R': T -> T -> state ATCDLang -> state ATCDLang -> Prop) s1 s2 lo,
+(forall n o1 o2 lo1,
+seln lo 0 [] = o1 ++ o2 ->
+Termination_Sensitive_explicit u (o1::lo1) s1 s2 p1 p2
 (Simulation.Definitions.compile
  ATCD_Refinement
  (Simulation.Definitions.compile
-    FD.refinement
-    (| Recover |)))
-(refines_valid ATCD_Refinement
- AD_valid_state) R
+ ATC_Refinement
+ File.recover))
+ (refines_valid ATCD_Refinement
+ (refines_valid ATC_Refinement
+AD_valid_state)) 
+R
 (ATCD_reboot_list n)) ->
 
-(forall n s1 s2 o s1' r1 s2' r2 ,
-exec ATCDLang u o s1 p1 (Finished s1' r1) ->
-exec ATCDLang u o s2 p2 (Finished s2' r2) ->
+(forall n s1' r1 s2' r2 o1 o2 lo2,
+seln lo 0 [] = o1 ++ o2 ->
+exec ATCDLang u o1 s1 p1 (Finished s1' r1) ->
+exec ATCDLang u o1 s2 p2 (Finished s2' r2) ->
 R s1 s2 ->
-Termination_Sensitive_explicit u s1' s2' (p3 r1) (p4 r2)
+Termination_Sensitive_explicit u (o2 :: lo2) s1' s2'
+(p3 r1) (p4 r2)
 (Simulation.Definitions.compile
 ATCD_Refinement
 (Simulation.Definitions.compile
-  FD.refinement
-  (| Recover |)))
-(refines_valid ATCD_Refinement
-AD_valid_state)
-R'
+ ATC_Refinement
+ File.recover))
+  (refines_valid ATCD_Refinement
+  (refines_valid ATC_Refinement
+ AD_valid_state))
+(R' r1 r2)
 (ATCD_reboot_list n)) ->
 
-
-(forall s1 s2 o s1' r1 s2' r2 ,
-exec ATCDLang u o s1 p1 (Finished s1' r1) ->
-exec ATCDLang u o s2 p2 (Finished s2' r2) ->
+(forall s1' r1 s2' r2 o1 o2,
+seln lo 0 [] = o1 ++ o2 ->
+exec ATCDLang u o1 s1 p1 (Finished s1' r1) ->
+exec ATCDLang u o1 s2 p2 (Finished s2' r2) ->
 R s1 s2 ->
-R' s1' s2') ->
+R' r1 r2 s1' s2') ->
 
-Termination_Sensitive_explicit u s1 s2 
+Termination_Sensitive_explicit u lo s1 s2
 (Bind p1 p3) (Bind p2 p4)
 (Simulation.Definitions.compile
 ATCD_Refinement
 (Simulation.Definitions.compile
-  FD.refinement
-  (| Recover |)))
-(refines_valid ATCD_Refinement
-AD_valid_state)
+ ATC_Refinement
+ File.recover))
+ (refines_valid ATCD_Refinement
+ (refines_valid ATC_Refinement
+AD_valid_state))
 R
 (ATCD_reboot_list n).
 Proof.
@@ -612,23 +220,24 @@ repeat invert_exec.
 invert_exec'' H12.
 edestruct H.
 4: eauto.
-all: eauto.
+all: simpl; eauto.
 instantiate (1 := RFinished _ _).
-instantiate (3 := 0).
+instantiate (3 := []).
 simpl.
 econstructor; eauto.
+
 eauto.
 simpl in *; invert_exec.
 
-edestruct H0.
-3: eauto.
-6: eauto.
+edestruct H0; cleanup.
+4: eauto.
+7: eauto.
 all: eauto.
 all: unfold refines_valid, AD_valid_state; simpl;
      unfold refines_valid, FD_valid_state; simpl; eauto.
 
 instantiate (1 := RFinished _ _).
-instantiate (3 := 0).
+instantiate (3 := []).
 simpl.
 econstructor; eauto.
 simpl in *; invert_exec.
@@ -648,21 +257,21 @@ invert_exec'' H15.
 {
   edestruct H.
   4: eauto.
-  all: eauto.
+  all: simpl; eauto.
   instantiate (1 := RFinished _ _).
-  instantiate (3 := 0).
+  instantiate (3 := []).
   simpl.
   econstructor; eauto.
   simpl in *; invert_exec.
   edestruct H0.
-3: eauto.
-6: eauto.
+4: eauto.
+7: eauto.
 all: eauto.
 all: unfold refines_valid, AD_valid_state; simpl;
      unfold refines_valid, FD_valid_state; simpl; eauto.
 
 instantiate (1 := Recovered _).
-instantiate (2 := S n).
+instantiate (2 := t::n).
 simpl.
 econstructor; eauto.
 simpl in *; invert_exec.
@@ -672,11 +281,14 @@ eexists (Recovered _); repeat econstructor; eauto.
 {
   edestruct H.
   4: eauto.
-  all: eauto.
+  all: simpl; eauto.
+  rewrite app_nil_r; eauto.
+
   instantiate (1 := Recovered _).
-  instantiate (2 := S n).
+  instantiate (2 := t::n).
   simpl.
   econstructor; eauto.
+  
   simpl in *; invert_exec.
   eexists (Recovered _); repeat econstructor; eauto.
 }
@@ -684,18 +296,22 @@ eexists (Recovered _); repeat econstructor; eauto.
 Unshelve.
 all: try solve [exact (fun _ _ => True)].
 all: simpl; eauto.
-Qed.
+all: try solve [exact []].
+all: try solve [exact Log.header0].
+all: try solve [exact Log.Current_Part].
+all: admit. (* These are Log Cache crashed then reboot implies other stuff things *)
+Admitted.
 
 
 Lemma ATCD_TS_ret:
-    forall n u T (t1 t2: T) V R,
+    forall n u T (t1 t2: T) V txns1 txns2 hdr1 hdr2,
     Termination_Sensitive u (Ret t1) (Ret t2)
-  (Simulation.Definitions.compile
-     ATCD_Refinement
-     (Simulation.Definitions.compile
-        FD.refinement
-        (| Recover |)))
-  V R
+    (Simulation.Definitions.compile
+    ATCD_Refinement
+    (Simulation.Definitions.compile
+     ATC_Refinement
+     File.recover))
+  V (equivalent_for_recovery txns1 txns2 Log.Current_Part hdr1 hdr2)
   (ATCD_reboot_list n).
   Proof.
     unfold Termination_Sensitive, ATCD_reboot_list; simpl; intros.
@@ -709,12 +325,6 @@ Lemma ATCD_TS_ret:
     all: unfold AD_valid_state, 
     refines_valid, FD_valid_state; 
     intros; simpl; eauto.
-    shelve.
+    eapply equivalent_for_recovery_after_reboot; eauto.
     eexists (Recovered _); repeat econstructor; eauto.
-    Unshelve.
-    all: try solve [exact (fun _ _ => True)].
-    all: simpl; eauto.
-
-    
-
   Qed.
