src/Noninterference/LoggedDisk/TS/TSRecovery/ATCD_TS_Recovery.v
@@ -1,0 +1,4 @@
+Require Export ATCD_TS_BatchOperations_Recovery.
+Require Export ATCD_TS_Log_Recovery.
+Require Export ATCD_TS_LogCache_Recovery.
+Require Export ATCD_TS_Common_Recovery.
